theories/Substitution/Introductions/Reflect.v
@@ -6,6 +6,25 @@ From LogRel.Substitution Require Import Irrelevance Properties SingleSubst.
 From LogRel.Substitution.Introductions Require Import Universe Var Nat SimpleArr Sigma Id Quote.
 
 Set Universe Polymorphism.
+Set Printing Primitive Projection Parameters.
+
+Section ToProve.
+
+(** TODO: consequences of confluence *)
+Axiom dred_tApp_qNat_closed0 : forall t t₀ n r₀,
+  [t ⇶* t₀] -> [tApp t (qNat n) ⇶* r₀] -> dnf t₀ -> dnf r₀ ->
+  closed0 t₀ -> closed0 r₀.
+
+Axiom dred_tApp_qNat_compat : forall t t₀ n m,
+  [t ⇶* t₀] -> dnf t₀ ->
+  [tApp t (qNat n) ⇶* qNat m] ->
+  [tApp t₀ (qNat n) ⇶* qNat m].
+
+(** Obviously true but annoying to prove *)
+Axiom dred_erase_qNat_compat : forall t n,
+  [t ⇶* qNat n] -> [erase t ⇶* qNat n].
+
+End ToProve.
 
 Section Utils.
 
@@ -24,87 +43,123 @@ Proof.
 destruct l; tea; now eapply (embRedTy Oi).
 Defined.
 
+Lemma ElURed {Γ A} (rU : [Γ ||-<one> U]) (rA : [rU | Γ ||- A : U]) : [Γ ||-<one> A].
+Proof.
+assert (rΓ : [|- Γ]) by now eapply wfc_wft, escape.
+unshelve (eapply LRTmRedIrrelevant' in rA; [|reflexivity]); [|apply (LRU_ (redUOne rΓ))|].
+destruct rA.
+apply (embRedTyOne rel).
+Qed.
+
+Lemma ElURedEq {Γ A A'} rΓ (rU := LRU_ (redUOne rΓ)) (rA : [Γ ||-<one> A]) (rAA' : [rU | Γ ||- A ≅ A' : U]) : [rA | Γ ||- A ≅ A'].
+Proof.
+destruct rAA'.
+unshelve (irrelevance0; [reflexivity|]).
+* shelve.
+* refine (embRedTyOne relL).
+* apply relEq.
+Qed.
+
+Lemma simple_AppRedEq {Γ t t' u u' F G l} (RF : [Γ ||-< l > F]) (RG : [Γ ||-< l > G]) (RΠ := SimpleArr.ArrRedTy RF RG) :
+  [RΠ | Γ ||- t ≅ t' : arr F G] -> [RF | Γ ||- u ≅ u' : F] -> [RG | Γ ||- tApp t u ≅ tApp t' u' : G].
+Proof.
+intros.
+eapply SimpleArr.simple_appcongTerm; tea.
++ now eapply LRTmEqRed_l.
++ now eapply LRTmEqRed_r.
+Qed.
+
 Lemma dnf_closed_qNat_aux : forall Γ (rNat : [Γ ||-Nat tNat]),
-  (forall t, [Γ ||-Nat t : tNat | rNat] -> forall u, [t ⇶* u] -> dnf u -> closed0 u -> ∑ n, u = qNat n) ×
-  (forall t, NatProp rNat t -> forall u, [t ⇶* u] -> dnf u -> closed0 u -> ∑ n, u = qNat n).
+  (forall t, [Γ ||-Nat t : tNat | rNat] -> forall u, [t ⇶* u] -> dnf u -> closed0 u -> ∑ n, u = qNat n × [Γ ||-Nat t ≅ qNat n : tNat | rNat]) ×
+  (forall t, NatProp rNat t -> forall u, [t ⇶* u] -> dnf u -> closed0 u -> ∑ n, u = qNat n × [Γ ||-Nat t ≅ qNat n : tNat | rNat]).
 Proof.
 intros; apply NatRedInduction.
 + intros * [? Hr] Heq ? IH u Hr' Hnf Hc.
-  apply IH; tea.
-  eapply dred_red_det; tea.
-  now eapply dred_red, redtm_sound.
+  unshelve epose (Hu := IH u _ _ _); tea.
+  { eapply dred_red_det; tea.
+    now eapply dred_red, redtm_sound. }
+  destruct Hu as (n&Hu&Hn).
+  exists n; split; tea.
+  change [LRNat_ one rNat | Γ ||- t ≅ qNat n : tNat].
+  eapply transEqTerm; [|tea].
+  eapply redSubstTerm; [|tea].
+  econstructor; tea.
+  now apply redtmwf_refl.
 + intros * Hr Hnf Hc.
   apply dred_dnf in Hr; [subst|eauto using dnf].
-  exists 0; reflexivity.
+  exists 0; split; [reflexivity|].
+  eapply (zeroRedEq (l := zero)).
+  now eapply wfc_wft, (escape (l := one)), LRNat_.
 + intros * Hn IH u Hr Hnf Hc.
   destruct (redalg_succ_adj _ _ Hr) as [m ->].
   apply redalg_succ_inv in Hr.
   inversion Hnf; subst; [|match goal with H : dne _ |- _ => inversion H end].
-  destruct (IH _ Hr) as [v Hv]; tea; subst.
-  exists (S v); reflexivity.
+  destruct (IH _ Hr) as (v&Hv&Hm); tea; subst.
+  exists (S v); split; [reflexivity|].
+  change [LRNat_ one rNat | Γ ||- tSucc n ≅ qNat (S v) : tNat].
+  change [LRNat_ one rNat | Γ ||- n ≅ qNat v : tNat] in Hm.
+  cbn; eapply succRedEq; tea.
+  now eapply LRTmEqRed_r.
 + intros n [? Hne] * Hr Hnf Hc; exfalso.
   apply convneu_whne in Hne.
   eapply dredalg_whne in Hr; [|tea].
   now eapply closed0_whne.
 Qed.
 
-Lemma dnf_closed_qNat : forall Γ l t u (rΓ : [|- Γ]) (rNat := natRed rΓ),
-  [Γ ||-<l> t : tNat | rNat] -> [t ⇶* u] -> dnf u -> closed0 u -> ∑ n, u = qNat n.
+Lemma dnf_closed_qNat : forall Γ l t u (rNat : [Γ ||-<l> tNat]),
+  [Γ ||-<l> t : tNat | rNat] -> [t ⇶* u] -> dnf u -> closed0 u -> ∑ n, (u = qNat n) × [rNat | Γ ||- t ≅ qNat n : tNat].
 Proof.
-intros * Ht Hr Hnf.
-edestruct dnf_closed_qNat_aux as [Haux ?]; eapply Haux; tea.
+intros * rt Hr Hnf **.
+assert (rΓ : [|- Γ]) by now eapply wfc_wft, escape.
+unshelve (eapply LRTmRedIrrelevant' in rt; [|reflexivity]); [|now apply (natRed (l := l))|].
+eapply dnf_closed_qNat_aux in rt; tea.
+destruct rt as (n&?&?).
+exists n; split; tea.
+unshelve (irrelevance0; [reflexivity|tea]); [|apply LRNat_|]; tea.
 Qed.
 
-Set Printing Primitive Projection Parameters.
-
-Lemma NatPropEq_diag {Γ A} {rNat : [Γ ||-Nat A]} :
-  (forall t u, [Γ ||-Nat t ≅ u : A | rNat] -> NatRedTm rNat t)
-  × (forall t u, NatPropEq rNat t u -> [Γ |- t : tNat] -> NatProp rNat t).
+Lemma dnf_closed_qNatRedEq : forall Γ l t n (rNat : [Γ ||-<l> tNat]),
+  [Γ ||-<l> t : tNat | rNat] -> [t ⇶* qNat n] -> [rNat | Γ ||- t ≅ qNat n : tNat].
 Proof.
+intros * rt Hred.
+eapply dnf_closed_qNat in rt; [|tea|apply dnf_qNat|apply closedn_qNat].
+destruct rt as (m&Hm&Hrt).
+apply qNat_inj in Hm; now subst m.
+Qed.
+
+Lemma dred_qNatRedEq {Γ l t n} (rNat : [Γ ||-<l> tNat]) :
+  [rNat | Γ ||- t ≅ qNat n : tNat] -> [t ⇶* qNat n].
+Proof.
+intros rEq.
+assert (rΓ : [|- Γ]) by now eapply wfc_wft, escape.
+assert (NN : [Γ ||-Nat tNat]).
+{ now constructor; apply redtywf_refl, wft_nat. }
+unshelve (eapply LRTmEqIrrelevant' in rEq; [|reflexivity]); [|now apply (LRNat_ l NN)|].
+enough (IH :
+(forall (t u : term), [Γ ||-Nat t ≅ u : tNat | NN] -> forall n, u = qNat n -> [t ⇶* qNat n])
+× (forall (t u : term), NatPropEq NN t u -> forall n, u = qNat n -> [t ⇶* qNat n])
+).
+{ destruct IH as [IH _]; eapply IH; [|reflexivity]; apply rEq. }
 apply NatRedEqInduction.
-+ intros; econstructor; tea.
-  - now eapply lrefl.
-  - destruct redL; eauto.
-+ constructor.
-+ intros; now constructor.
-+ intros * []; constructor.
-  constructor; tea; now eapply lrefl.
++ intros ???????? IH **; subst.
+  etransitivity.
+  - now eapply dred_red, redtm_sound, tmr_wf_red.
+  - apply IH; symmetry; apply red_whnf;
+    eauto using dnf_whnf, dnf_qNat, tmr_wf_red, redtm_sound.
++ intros []; cbn; [reflexivity|congruence].
++ intros ??? IH []; cbn; try congruence.
+  intros [=]; now apply dredalg_succ, IH.
++ intros ?? [] m' **; subst; exfalso.
+  assert (Hne : whne (qNat m')) by now (eapply convneu_whne; symmetry).
+  destruct m'; inversion Hne.
 Qed.
 
-Lemma LRTmEqRed_l : forall Γ l A t u (rA : [Γ ||-<l> A]),
-  [rA | Γ ||- t ≅ u : A] -> [rA | Γ ||- t : A].
+Lemma red_qNat_inj {Γ l m n} (rNat : [Γ ||-<l> tNat]) :
+  [rNat | Γ ||- qNat m ≅ qNat n : tNat] -> m = n.
 Proof.
-intros Γ l A t u rA.
-revert t u.
-pattern l, Γ, A, rA.
-eapply Induction.LR_rect_TyUr; clear l Γ A rA.
-+ intros l Γ A rU t u [rl]; apply rl.
-+ intros l Γ A rne t u [].
-  unshelve econstructor; [|tea|].
-  now eapply lrefl.
-+ intros l Γ A rΠ IHdom IHcod t u []; tea.
-+ intros l Γ A rNat t u [].
-  cbn; econstructor; [tea| |].
-  - now eapply lrefl.
-  - destruct redL; now eapply NatPropEq_diag.
-+ intros l Γ A rEmpty t u [].
-  cbn; econstructor; [tea| |].
-  - now eapply lrefl.
-  - destruct prop; do 2 constructor.
-    * apply redL.
-    * destruct r; now eapply lrefl.
-+ intros l Γ A rΣ IHdom IHcod t u []; tea.
-+ intros l Γ A rId IHty IHty' t u [].
-  cbn; econstructor; [tea| |].
-  - now eapply lrefl.
-  - destruct prop; [left|right]; tea.
-    split; [apply redL|destruct r; now eapply lrefl].
-Qed.
-
-Lemma LRTmEqRed_r : forall Γ l A t u (rA : [Γ ||-<l> A]),
-  [rA | Γ ||- t ≅ u : A] -> [rA | Γ ||- u : A].
-Proof.
-intros; now eapply LRTmEqRed_l, LRTmEqSym.
+intros rEq.
+apply qNat_inj, dred_dnf; [|apply dnf_qNat].
+now apply dred_qNatRedEq in rEq.
 Qed.
 
 Lemma red_redtm_exp {Γ l A t t' u u'} (rA : [Γ ||-<l> A]) :
@@ -118,6 +173,16 @@ eapply transEqTerm; [|eapply transEqTerm; [|apply LRTmEqSym]].
 - tea.
 - apply redSubstTerm; [|tea].
   now eapply LRTmEqRed_r.
+Qed.
+
+Lemma neuTermEqRed {Γ l A t t' n n'} (RA : [Γ ||-<l> A]) :
+  [Γ |- t ⤳* n : A] ->
+  [Γ |- t' ⤳* n' : A] ->
+  [Γ |- n : A] -> [Γ |- n' : A] -> [Γ |- n ~ n' : A] -> [Γ ||-<l> t ≅ t' : A | RA].
+Proof.
+intros Ht Ht' Hn Hn' Hnn'.
+eapply red_redtm_exp; tea.
+now eapply neuTermEq.
 Qed.
 
 Lemma simple_betaRed {Γ l A B t a} (rΓ : [|- Γ])
@@ -372,6 +437,88 @@ unshelve econstructor.
     * apply relEq.
 Qed.
 
+Lemma simple_tPairRed {Γ l A B p q}
+  (rA : [Γ ||-<l> A]) (rB : [Γ ||-<l> B])
+  (rΣ : [Γ ||-<l> tAnd A B])
+  (rp : [rA | Γ ||- p : A]) (rq : [rB | Γ ||- q : B]) : [rΣ | Γ ||- tPair A B⟨↑⟩ p q : tAnd A B].
+Proof.
+pose (rΣ0 := normRedΣ rΣ).
+unshelve (irrelevance0; [reflexivity|]); [|apply rΣ0|].
+assert [|- Γ] by now eapply wfc_wft, escape.
+assert [Γ |- A] by now eapply escape.
+assert [|- Γ,, A] by gen_typing.
+assert [Γ |- B] by now eapply escape.
+assert [Γ,, A |- B⟨↑⟩].
+{ rewrite <- (@wk1_ren_on Γ A); tea; eapply wft_wk; gen_typing. }
+assert [Γ |- p : A] by now eapply escapeTerm.
+assert [Γ |- q : B] by now eapply escapeTerm.
+assert [Γ |- tPair A B⟨↑⟩ p q : tSig A B⟨↑⟩].
+{ apply ty_pair; tea.
+  now replace  B⟨↑⟩[p..] with B by now bsimpl. }
+assert [Γ |- A ≅ A] by now unshelve eapply escapeEq, reflLRTyEq.
+assert [Γ |- B ≅ B] by now unshelve eapply escapeEq, reflLRTyEq.
+assert [Γ |- p ≅ p : A] by now unshelve eapply escapeEqTerm, reflLRTmEq.
+assert [Γ |- q ≅ q : B] by now unshelve eapply escapeEqTerm, reflLRTmEq.
+assert [Γ,, A |- B⟨↑⟩ ≅ B⟨↑⟩].
+{ rewrite <- (@wk1_ren_on Γ A).
+  now apply convty_wk. }
+assert (Hrw : forall x ρ, B⟨↑⟩[x .: ρ >> tRel] = B⟨ρ⟩).
+{ intros. bsimpl; symmetry; apply rinstInst'_term. }
+assert [Γ |- tSnd (tPair A B⟨↑⟩ p q) ⤳* q : B].
+{ set (B' := B) at 1.
+  replace B' with B⟨↑⟩[(tFst (tPair A B⟨↑⟩ p q))..] by now bsimpl.
+  clear B'; eapply redtm_snd_beta; tea.
+  now replace B⟨↑⟩[p..] with B by now bsimpl. }
+unshelve econstructor.
++ exact (tPair A B⟨↑⟩ p q).
++ intros.
+  assert [Δ |- A⟨ρ⟩] by now apply wft_wk.
+  eapply redSubstTerm; cbn; [|apply redtm_fst_beta]; tea.
+  - irrelevance0; [reflexivity|]; now apply wkTerm.
+  - rewrite <- wk_up_ren_on with (F := A).
+    apply wft_wk; [apply wfc_cons|]; tea.
+  - now eapply ty_wk.
+  - let T := match goal with |- [_ |- _ : ?T] => T end in
+    replace T with B⟨ρ⟩.
+    2:{ bsimpl; apply rinstInst'_term. }
+    apply ty_wk; tea.
+  Unshelve. all: tea.
++ cbn; apply redtmwf_refl.
+  apply ty_pair; tea.
+  - let T := match goal with |- [_ |- _ : ?T] => T end in
+    replace T with B by now bsimpl.
+    tea.
++  unshelve econstructor; cbn.
+  - intros.
+    irrelevance0; [reflexivity|].
+    unshelve apply wkTerm, rp; tea.
+  - intros.
+    unshelve (irrelevance0; [reflexivity|]); [shelve|..].
+    * now unshelve apply wk, rA.
+    * unshelve apply reflLRTyEq.
+  - intros.
+    rewrite Hrw.
+    irrelevance0; [symmetry; apply Hrw|].
+    now unshelve apply wkEq, reflLRTyEq.
+  - intros.
+    irrelevance0; [symmetry; apply Hrw|].
+    now unshelve apply wkTerm.
++ assert (isWfPair Γ A B⟨↑⟩ (tPair A B⟨↑⟩ p q)).
+  { constructor; tea; now replace B⟨↑⟩[p..] with B by now bsimpl. }
+  cbn; eapply convtm_eta_sig; tea.
+  - assert [Γ |- tFst (tPair A B⟨↑⟩ p q) ⤳* p : A].
+    { apply redtm_fst_beta; tea.
+      now replace B⟨↑⟩[p..] with B by now bsimpl. }
+    eapply convtm_exp; tea.
+  - match goal with |- [_ |- _ ≅ _ : ?T] => replace T with B by now bsimpl end.
+    eapply convtm_exp; tea.
++ intros; cbn.
+  unshelve (irrelevance0; [symmetry; apply Hrw|]); [|now unshelve apply wk|].
+  eapply redSubstTerm; [now eapply wkTerm|].
+  let H := match goal with H : [_ |- _  ⤳* _ : _ ] |- _ => H end in
+  eapply redtm_wk with (ρ := ρ) in H; [|tea]; apply H.
+Qed.
+
 Lemma tIsNilRed {Γ l t} (rΓ : [|- Γ])
   (rNat := natRed rΓ)
   (rU : [Γ ||-<one> U])
@@ -456,16 +603,13 @@ assert (rΓ : [|- Γ]).
 { eapply wfc_wft; now eapply escape. }
 pose (rNat := natRed (l := l) rΓ).
 unshelve eapply simple_lambdaRed; tea; intros.
-cbn - [rB]; unshelve eapply (SimpleArr.simple_appcongTerm (F := tNat)).
+cbn - [rB]; unshelve eapply (simple_AppRedEq (F := tNat)).
 + tea.
-+ change (arr tNat tNat⟨ρ⟩) with (arr tNat tNat)⟨ρ⟩.
-  now eapply (wk ρ).
 + assert (Hrw : forall a, t⟨ρ⟩ = t⟨↑⟩[a .: ρ >> tRel]).
   { intros; bsimpl; apply rinstInst'_term. }
   rewrite <- !Hrw.
-  now apply reflLRTmEq, wkTerm.
-+ eapply succRed; tea.
-+ eapply succRed; tea.
+  eapply reflLRTmEq, LRTmRedIrrelevant', wkTerm; [|tea]; reflexivity.
+  Unshelve. tea.
 + eapply succRedEq; tea.
 Qed.
 
@@ -613,7 +757,7 @@ apply neuTermEq.
 + apply tEval_cong; tea.
 Qed.
 
-Lemma tEvalRedEq {Γ l t t' k k' v v'} (rΓ : [|- Γ])
+Lemma tEvalURedEq {Γ l t t' k k' v v'} (rΓ : [|- Γ])
   (rNat : [Γ ||-<l> tNat]) (rPNat : [Γ ||-<l> tPNat])
   (rU : [Γ ||-<one> U])
   (rt : [Γ ||-<l> t ≅ t' : tPNat | rPNat])
@@ -683,38 +827,7 @@ apply NatRedEqInduction; unfold P.
   apply rk.
 Qed.
 
-(*
-Lemma tEvalZeroBranchRed {Γ v} (rΓ : [|- Γ])
-  (rNat : [Γ ||-<one> tNat]) (rP : [Γ ||-<one> arr tPNat U])
-  (rv : [rNat | Γ ||- v : tNat]) :
-  [rP | Γ ||- tLambda tPNat (tIsVal (tApp (tRel 0) tZero) v⟨↑⟩) : arr tPNat U].
-Proof.
-unshelve eapply simple_lambdaRed; tea.
-+ apply SimpleArr.ArrRedTy; now apply natRed.
-+ now apply LRU_, redUOne.
-+ intros.
-  rewrite !tIsVal_subst; cbn - [rB].
-  assert (Hrw : forall a, v⟨↑⟩[a .: ρ >> tRel] = v⟨ρ⟩).
-  { intros x; bsimpl; symmetry; apply rinstInst'_term. }
-  rewrite !Hrw.
-Admitted.
-
-Lemma tEvalSuccBranchRed {Γ} (rΓ : [|- Γ]) (rS : [Γ ||-<one> arr tNat (arr (arr tPNat U) (arr tPNat U))]) :
-  [rS | Γ ||- tLambda tNat (tLambda (arr tPNat U) (tLambda tPNat
-    (tAnd (tIsNil (tApp (tRel 0) (tRel 2))) (tApp (tRel 1) (tShift (tRel 0)))))) : arr tNat (arr (arr tPNat U) (arr tPNat U))].
-Proof.
-unshelve eapply simple_lambdaRed; tea.
-+ now apply natRed.
-+ do 2 apply SimpleArr.ArrRedTy; admit.
-+ intros.
-  cbn - [tAnd tIsNil].
-  rewrite !tAnd_subst, !tIsNil_subst.
-  cbn - [tAnd tIsNil].
-  admit.
-Admitted.
-*)
-
-Lemma tEvalRed {Γ l t k v} (rΓ : [|- Γ])
+Lemma tEvalURed {Γ l t k v} (rΓ : [|- Γ])
   (rNat := natRed rΓ) (rNatNat := SimpleArr.ArrRedTy rNat rNat)
   (rU : [Γ ||-<one> U])
   (rt : [Γ ||-<l> t : tPNat | rNatNat])
@@ -722,14 +835,14 @@ Lemma tEvalRed {Γ l t k v} (rΓ : [|- Γ])
   (rv : [Γ ||-<l> v : tNat | rNat]) :
   [Γ ||-<one> tEval t k v : U | rU].
 Proof.
-eapply LRTmEqRed_l, tEvalRedEq.
+eapply LRTmEqRed_l, tEvalURedEq.
 + tea.
 + now eapply reflLRTmEq.
 + now eapply reflLRTmEq.
 + now eapply reflLRTmEq.
 Qed.
 
-Lemma tEvalRedTy {Γ l t k v} (rΓ : [|- Γ])
+Lemma tEvalRed {Γ l t k v} (rΓ : [|- Γ])
   (rNat := natRed rΓ) (rNatNat := SimpleArr.ArrRedTy rNat rNat)
   (rt : [Γ ||-<l> t : tPNat | rNatNat])
   (rk : [Γ ||-<l> k : tNat | rNat])
@@ -739,8 +852,819 @@ Proof.
 unshelve epose (rU := LRU_ (redUOne _)); [|tea|].
 enough (rEval : [rU | Γ ||- tEval t k v : U]).
 { destruct rEval; apply (embRedTyOne rel). }
-eapply tEvalRed; tea.
+eapply tEvalURed; tea.
 Qed.
+
+Lemma qEvalTyURed {Γ} (rU : [Γ ||-< one > U]) k v: [rU | Γ ||- qEvalTy k v : U].
+Proof.
+assert (rΓ : [|- Γ]).
+{ now eapply wfc_wft, escape. }
+induction k; simpl.
++ unshelve eapply tIsValRed; [shelve|..].
+  - tea.
+  - unshelve eapply (succRed (l := one)), qNatRed.
+  - eapply qNatRed.
++ eapply tAndURed; [tea| |].
+  - now eapply tIsNilRed, zeroRed.
+  - tea.
+Unshelve. all: first [apply one|tea].
+Qed.
+
+Lemma qEvalTyRed {Γ} (rΓ : [|- Γ]) k v : [Γ ||-<one> qEvalTy k v].
+Proof.
+unshelve epose (rU := LRU_ (redUOne _)); [|tea|].
+enough (rEval : [rU | Γ ||- qEvalTy k v : U]).
+{ destruct rEval; apply (embRedTyOne rel). }
+eapply qEvalTyURed; tea.
+Qed.
+
+Lemma qEvalTmRed {Γ k v} (rΓ : [|- Γ]) : [qEvalTyRed rΓ k v | Γ ||- qEvalTm k v : qEvalTy k v].
+Proof.
+induction k; cbn.
++ unshelve eapply Id.reflRed.
+  - now eapply natRed.
+  - apply succRed, qNatRed.
++ assert (Hrw : qEvalTy (S k) v = tAnd (tId tNat tZero tZero) (qEvalTy k v)) by reflexivity.
+  pose (rNat := natRed (l := one) rΓ).
+  unshelve (irrelevance0; [symmetry; apply Hrw|]).
+  2:{ apply tAndRed; tea; [|now apply qEvalTyRed].
+      unshelve eapply Id.IdRed; [tea| |]; eapply zeroRed; tea. }
+  set (T := qEvalTy k v) at 2.
+  replace T with (qEvalTy k v)⟨↑⟩ by apply qEvalTy_ren.
+  unshelve eapply simple_tPairRed.
+  - unshelve eapply Id.IdRed; tea; eapply zeroRed; tea.
+  - now apply qEvalTyRed.
+  - unshelve eapply Id.reflRed.
+    * now apply natRed.
+    * now apply zeroRed.
+  - apply IHk.
+Qed.
+
+Lemma tShiftAppRedEq {Γ l t n} {rΓ : [|- Γ]}
+  (rNat := natRed (l := l) rΓ) (rPNat := SimpleArr.ArrRedTy rNat rNat) :
+  [rPNat | Γ ||- t : tPNat] -> [rNat | Γ ||- n : tNat] ->
+  [rNat | Γ ||- tApp (tShift t) n ≅ tApp t (tSucc n) : tNat].
+Proof.
+intros rt rn.
+eapply redSubstTerm; [|apply redtm_shift_app].
++ unshelve eapply (SimpleArr.simple_appTerm (F := tNat)); tea.
+  now apply succRed.
++ now eapply escapeTerm.
++ now eapply escapeTerm.
+Qed.
+
+Lemma qEvalTyRedEq {Γ t k v} (rΓ : [|- Γ]) (rU : [Γ ||-<one> U])
+  (rNat := natRed (l := one) rΓ) (rPNat := SimpleArr.ArrRedTy rNat rNat) :
+  [rPNat | Γ ||- t : tPNat] ->
+  (forall k', k' < k -> [rNat | Γ ||- tApp t (qNat k') ≅ tZero : tNat]) ->
+  [rNat | Γ ||- tApp t (qNat k) ≅ tSucc (qNat v) : tNat] ->
+  [rU | _ ||- tEval t (qNat k) (qNat v) ≅ qEvalTy k v : U ].
+Proof.
+revert t.
+induction k; cbn [qNat qEvalTy].
++ intros t Ht Hlt Hk.
+  eapply transEqTerm; [eapply tEvalZeroRedEq|].
+  - tea.
+  - apply qNatRed.
+  - eapply tIsValRedEq.
+    * apply Hk.
+    * apply qNatRedEq.
++ intros t Ht Hlt Hk.
+  assert [rNat | Γ ||- qNat k : tNat] by apply qNatRed.
+  assert [rNat | Γ ||- qNat v : tNat] by apply qNatRed.
+  assert [rPNat | Γ ||- tShift t : tPNat] by now apply tShiftRed.
+  assert [rU | Γ ||- tEval (tShift t) (qNat k) (qNat v) : U] by now eapply tEvalURed; tea.
+  eapply transEqTerm; [eapply tEvalSuccRedEq|]; tea.
+  apply tAndURedEq; tea.
+  - unshelve eapply tIsNilRedEq; [exact one|tea|].
+    apply Hlt; Lia.lia.
+  - apply IHk; tea.
+    * intros k' Hk'.
+      assert [rNat | Γ ||- qNat k' : tNat] by apply qNatRed.
+      eapply transEqTerm; [eapply tShiftAppRedEq|]; tea.
+      apply (Hlt (S k')); Lia.lia.
+    * eapply transEqTerm; [eapply tShiftAppRedEq|]; tea. 
+Qed.
+
+End Utils.
+
+Section StepRed.
+
+Context `{GenericTypingProperties}.
+Context {SN : SNTypingProperties ta _ _ _ _ _}.
+
+Lemma StepClosed0RedEq : forall Γ l t u k v (rΓ : [|- Γ]) (rNat := natRed rΓ),
+  [Γ ||-<l> run model : arr tNat (arr tNat tPNat) | SimpleArr.ArrRedTy rNat (SimpleArr.ArrRedTy rNat (SimpleArr.ArrRedTy rNat rNat))] ->
+  dnf t -> [Γ |- t ≅ t : arr tNat tNat] -> closed0 t -> EvalStep Γ t u k v ->
+  [rNat | Γ ||- tStep t (qNat u) ≅ qNat k : tNat].
+Proof.
+intros.
+eapply redSubstTerm.
++ eapply qNatRed.
++ eapply redtm_evalstep; tea.
+  now eapply escapeTerm.
+Qed.
+
+Lemma erase_qNat : forall n, erase (qNat n) = qNat n.
+Proof.
+induction n; cbn; now f_equal.
+Qed.
+
+Lemma eqnf_qRun {t t' u k} : eqnf t t' -> qRun t u k = qRun t' u k.
+Proof.
+intros Heq; unfold qRun.
+now rewrite Heq.
+Qed.
+
+Lemma unannot_qRun {t t' u k} : unannot t = unannot t' -> qRun t u k = qRun t' u k.
+Proof.
+intros Heq; unfold qRun.
+now rewrite !erase_unannot_etared, Heq.
+Qed.
+
+Lemma qRun_subst {t u k σ} : closed0 t -> (qRun t u k)[σ] = qRun t[σ] u k.
+Proof.
+intros Ht.
+rewrite (@unannot_qRun t[σ] t); [|now eapply unannot_closed0_subst].
+unfold qRun; cbn; rewrite !qNat_subst.
+now rewrite run_subst.
+Qed.
+
+Lemma eqnf_EvalStep {Γ t t' u k v} : eqnf t t' -> EvalStep Γ t u k v -> EvalStep Γ t' u k v.
+Proof.
+intros Heq [Hevl Hnil Hval]; split.
++ now rewrite <- Heq.
++ intros; erewrite <- eqnf_qRun; eauto.
++ erewrite <- eqnf_qRun; eauto.
+Qed.
+
+Lemma minimize (f : nat -> bool) (n : nat) :
+  is_true (f n) -> ∑ m, is_true (f m) × (forall m', m' < m -> ~ is_true (f m')).
+Proof.
+revert f; induction n; intros f Hn.
++ exists 0; split; [tea|Lia.lia].
++ destruct (IHn (fun n => f (S n)) Hn) as (m&Hm&Hlt).
+  remember (f 0) as b eqn:Hb; symmetry in Hb; destruct b.
+  - exists 0; split; [tea|Lia.lia].
+  - exists (S m); split; [tea|].
+    intros []; [congruence|].
+    intros; apply Hlt; Lia.lia.
+Qed.
+
+Lemma murec_intro {A} {f k v} :
+  (forall k', k' < k -> f k' = None) -> f k = Some v ->
+  @murec A f (S k) = Some (k, v).
+Proof.
+intros Hlt Hk; cbn.
+assert (Hrw : forall l, muget 0 (List.rev (muval f k) ++ l) = muget k l).
+{ revert Hlt; clear.
+  induction k; cbn; [reflexivity|].
+  intros Hlt l.
+  rewrite <- List.app_assoc; rewrite IHk; [|now eauto].
+  cbn; now rewrite Hlt. }
+rewrite Hrw; cbn; now rewrite Hk.
+Qed.
+
+Lemma murec_elim_None {A f k k₀ k' v} : k' < k -> @murec A f k₀ = Some (k, v) -> f k' = None.
+Proof.
+unfold murec.
+revert f v k k'.
+induction k₀ as [|k₀]; cbn; intros f v k k' Hlt Hrec.
+Admitted.
+
+Lemma murec_elim_Some {A f k k₀ v} : @murec A f k₀ = Some (k, v) -> f k = Some v.
+Proof.
+intros Hrec.
+induction k₀; cbn in *.
++ congruence.
++ 
+Admitted.
+
+Lemma dredalg_eval_min {deep t r} : @RedClosureAlg deep t r -> dnf r ->
+  ∑ k : nat, (forall k', k' < k -> eval deep t k' = None) × eval deep t k = Some r.
+Proof.
+intros Hred Hnf.
+assert (Heval0 := Hred); apply dredalg_eval in Heval0; [|tea].
+pose (f k := match eval deep t k with None => false | Some _ => true end).
+destruct Heval0 as [k0 Hk0].
+destruct (minimize f k0) as (k&Hk&Hlt); unfold f in *; clear f.
++ rewrite Hk0; reflexivity.
++ exists k; split.
+  - intros k' Hk'; specialize (Hlt k' Hk').
+    destruct (eval deep t k'); congruence.
+  - remember (eval deep t k) as w eqn:Hw; symmetry in Hw.
+    destruct w; [|congruence].
+    destruct (PeanoNat.Nat.le_ge_cases k k0).
+    * eapply eval_mon in Hw; [|tea]; congruence.
+    * eapply eval_mon in Hk0; [|tea]; congruence.
+Qed.
+
+Axiom run_spec_None : forall t u k,
+  eval true (tApp t (qNat u)) k = None ->
+  [tApp (tApp (tApp (run model) (qNat (quote model t))) (qNat u)) (qNat k) ⇶* tZero].
+
+Axiom run_spec_Some : forall t u k v,
+  eval true (tApp t (qNat u)) k = Some (qNat v) ->
+  [tApp (tApp (tApp (run model) (qNat (quote model t))) (qNat u)) (qNat k) ⇶* tSucc (qNat v)].
+
+Lemma reify_EvalStep {Γ l t n v} (rNat : [Γ ||-<l> tNat]) :
+  (forall k, [rNat | Γ ||- qRun t n k : tNat]) ->
+  [tApp t (qNat n) ⇶* qNat v] ->
+  ∑ k, EvalStep Γ t n k v.
+Proof.
+intros * Hrun Hred.
+assert (Hred' : [tApp (erase t) (qNat n) ⇶* qNat v]).
+{ apply dred_erase_qNat_compat in Hred; cbn in Hred.
+  now rewrite erase_qNat in Hred. }
+
+assert (Heval0 := Hred'); apply dredalg_eval in Heval0; [|apply dnf_qNat].
+assert (Heval : ∑ k,
+  (forall k', k' < k -> (eval true (tApp (erase t) (qNat n)) k' = None)) ×
+  (eval true (tApp (erase t) (qNat n)) k = Some (qNat v))).
+{ apply dredalg_eval_min; eauto using dnf_qNat. }
+destruct Heval as (k&Hnil&Heval).
+exists k; split.
++ exists (S k).
+  now apply murec_intro.
++ intros k' Hk'.
+  specialize (Hnil k' Hk').
+  apply run_spec_None in Hnil.
+  now eapply escapeEqTerm, dnf_closed_qNatRedEq with (n := 0).
++ apply run_spec_Some in Heval.
+  now eapply escapeEqTerm, dnf_closed_qNatRedEq with (n := (S v)).
+Qed.
+
+Lemma StepRedEq : forall Γ l t t' u u' (rΓ : [|- Γ]) (rNat := natRed rΓ) (rNatNat := SimpleArr.ArrRedTy rNat rNat),
+  [Γ ||-<l> t ≅ t' : arr tNat tNat | rNatNat ] ->
+  [Γ ||-<l> u ≅ u' : tNat | rNat ] ->
+  [Γ ||-<l> run model : arr tNat (arr tNat tPNat) | SimpleArr.ArrRedTy rNat (SimpleArr.ArrRedTy rNat rNatNat)] ->
+  [Γ ||-<l> tStep t u ≅ tStep t' u' : tNat | rNat ].
+Proof.
+intros * rtt' ruu' rrun.
+assert (rt : [Γ ||-<l> t : arr tNat tNat | rNatNat ]) by now eapply LRTmEqRed_l.
+assert (rt' : [Γ ||-<l> t' : arr tNat tNat | rNatNat ]) by now eapply LRTmEqRed_r.
+assert (ru : [Γ ||-<l> u : tNat | rNat ]) by now eapply LRTmEqRed_l.
+assert (ru' : [Γ ||-<l> u' : tNat | rNat ]) by now eapply LRTmEqRed_r.
+assert [Γ |- run model : arr tNat (arr tNat tPNat)] by now eapply escapeTerm.
+assert (Hnft := rtt'); apply escapeEqTerm, snty_nf in Hnft.
+assert (Hnfu := ruu'); apply escapeEqTerm, snty_nf in Hnfu.
+destruct Hnft as (t₀&t'₀&[]&[]&?&?&?).
+destruct Hnfu as (u₀&u'₀&[]&[]&?&?&?).
+remember (is_closedn 0 t₀) as ct eqn:Hct; symmetry in Hct.
+assert (Hct' : is_closedn 0 t'₀ = ct).
+{ erewrite eqnf_is_closedn; [tea|now apply Symmetric_eqnf]. }
+remember (is_closedn 0 u₀) as cu eqn:Hcu; symmetry in Hcu.
+assert (Hcu' : is_closedn 0 u'₀ = cu).
+{ erewrite eqnf_is_closedn; [tea|now apply Symmetric_eqnf]. }
+remember (andb ct cu) as cb eqn:Hcb; symmetry in Hcb; destruct cb.
++ destruct ct; [|cbn in Hcb; congruence].
+  destruct cu; [|cbn in Hcb; congruence].
+  clear Hcb.
+
+  assert (∑ n₀, u₀ = qNat n₀ ×  [rNat | Γ ||- u ≅ qNat n₀ : tNat]) as (n₀&?&?) by now eapply dnf_closed_qNat.
+  assert (∑ n'₀, u'₀ = qNat n'₀ ×  [rNat | Γ ||- u' ≅ qNat n'₀ : tNat]) as (n'₀&?&?) by now eapply dnf_closed_qNat.
+  subst.
+  assert (n₀ = n'₀); [|subst n'₀].
+  { eapply red_qNat_inj, transEqTerm, transEqTerm; [now apply LRTmEqSym| |tea]; tea. }
+
+  assert (rvv' : [rNat | Γ ||- tApp t (qNat n₀) ≅ tApp t' (qNat n₀) : tNat]).
+  { unshelve eapply (LogicalRelation.SimpleArr.simple_appcongTerm (F := tNat)); tea; first [apply qNatRed|apply qNatRedEq]. }
+
+  assert (Hnfv := rvv'); apply escapeEqTerm, snty_nf in Hnfv.
+  destruct Hnfv as (v₀&v'₀&[]&[]&?&?&?).
+
+  assert (rv : [rNat | Γ ||- tApp t (qNat n₀) : tNat]) by now eapply LRTmEqRed_l.
+  assert (rv' : [rNat | Γ ||- tApp t' (qNat n₀) : tNat]) by now eapply LRTmEqRed_r.
+
+
+  assert (∑ m₀, v₀ = qNat m₀ ×  [rNat | Γ ||- tApp t (qNat n₀) ≅ qNat m₀ : tNat]) as (m₀&?&?).
+  { eapply dnf_closed_qNat; tea.
+    eapply (dred_tApp_qNat_closed0 t t₀ n₀); eauto. }
+  assert (∑ m₀, v'₀ = qNat m₀ ×  [rNat | Γ ||- tApp t' (qNat n₀) ≅ qNat m₀ : tNat]) as (m'₀&?&?).
+  { eapply dnf_closed_qNat; tea.
+    eapply (dred_tApp_qNat_closed0 t' t'₀ n₀); eauto. }
+  subst.
+
+  subst.
+  let H := match goal with H : eqnf (qNat _) (qNat _) |- _ => H end in
+  unfold eqnf in H; rewrite !erase_qNat in H; apply qNat_inj in H; subst m'₀.
+
+  assert (forall k : nat, [rNat | Γ ||- qRun t₀ n₀ k : tNat]).
+  { intros k; unfold qRun.
+    unshelve eapply (SimpleArr.simple_appTerm (F := tNat)); tea; [|apply qNatRed].
+    assert (rT : [Γ ||-< l > arr tNat (arr tNat tNat)]) by now apply SimpleArr.ArrRedTy.
+    unshelve eapply (SimpleArr.simple_appTerm (F := tNat)); tea; [|apply qNatRed].
+    unshelve eapply (SimpleArr.simple_appTerm (F := tNat)); tea; apply qNatRed.
+  }
+
+  assert (∑ k, EvalStep Γ t₀ n₀ k m₀) as [k Hk].
+  { eapply reify_EvalStep; [tea|].
+    now eapply dred_tApp_qNat_compat. }
+
+  eapply red_redtm_exp; try eapply redtm_step; tea.
+  eapply red_redtm_exp; try eapply redtm_evalstep; tea.
+  - now eapply urefl.
+  - now eapply urefl.
+  - eapply eqnf_EvalStep; tea.
+  - apply qNatRedEq.
++ eapply neuTermEqRed.
+  - now eapply redtm_step.
+  - now eapply redtm_step.
+  - apply ty_step; tea; now eapply urefl.
+  - apply ty_step; tea; now eapply urefl.
+  - eapply convneu_step; tea.
+    * etransitivity; [now symmetry|].
+      etransitivity; [now eapply escapeEqTerm|tea].
+    * etransitivity; [now symmetry|].
+      etransitivity; [now eapply escapeEqTerm|tea].
+    * now symmetry.
+    * now symmetry.
+    * rewrite Hct, Hcu; destruct ct, cu; compute; now eauto.
+    * rewrite Hct', Hcu'; destruct ct, cu; compute; now eauto.
+Qed.
+
+Lemma StepRed : forall Γ l t u (rΓ : [|- Γ]) (rNat := natRed rΓ) (rNatNat := SimpleArr.ArrRedTy rNat rNat),
+  [Γ ||-<l> t : arr tNat tNat | rNatNat ] ->
+  [Γ ||-<l> u : tNat | rNat ] ->
+  [Γ ||-<l> run model : arr tNat (arr tNat tPNat) | SimpleArr.ArrRedTy rNat (SimpleArr.ArrRedTy rNat rNatNat)] ->
+  [Γ ||-<l> tStep t u : tNat | rNat ].
+Proof.
+intros.
+eapply LRTmEqRed_l, StepRedEq.
++ apply reflLRTmEq; tea.
++ apply reflLRTmEq; tea.
++ tea.
+Qed.
+
+Lemma reify_red_EvalStep {Γ l t u k v v'} (rNat : [Γ ||-<l> tNat]) :
+  (forall k' : nat, k' < k -> [rNat | Γ ||- qRun t u k' ≅ tZero : tNat]) ->
+  [rNat | Γ ||- qRun t u k ≅ tSucc (qNat v) : tNat] ->
+  [tApp t (qNat u) ⇶* qNat v'] ->
+  EvalStep Γ t u k v.
+Proof.
+intros rnil rval Hred.
+split.
++ assert (Hered := Hred).
+  apply dred_erase_qNat_compat in Hered; cbn in Hered.
+  rewrite erase_qNat in Hered.
+  assert (pnil : forall k', k' < k -> [qRun t u k' ⇶* tZero]).
+  { intros; now eapply (dred_qNatRedEq (n := 0)). }
+  assert (pval : [qRun t u k ⇶* tSucc (qNat v)]).
+  { intros; now eapply (dred_qNatRedEq (n := (S v))). }
+  clear rNat rnil rval.
+  apply dredalg_eval_min in Hered as (k₀&Hnil&Hval); [|apply dnf_qNat].
+  assert (Henil : forall k', k' < k₀ -> [qRun t u k' ⇶* tZero]).
+  { intros; now apply run_spec_None, Hnil. }
+  assert (Heval : [qRun t u k₀ ⇶* tSucc (qNat v')]) by now apply run_spec_Some.
+  assert (k = k₀); [|subst k₀].
+  { destruct (PeanoNat.Nat.lt_trichotomy k k₀) as [|[|]]; [|now tea|]; exfalso.
+    + unshelve epose (Henil k _); tea.
+      assert (tZero = tSucc (qNat v)); [|congruence].
+      eapply dredalg_det; tea; eauto using dnf, dnf_qNat.
+    + unshelve epose (pnil k₀ _); tea.
+      assert (tZero = tSucc (qNat v')); [|congruence].
+      eapply dredalg_det; eauto using dnf, dnf_qNat. }
+  assert (tSucc (qNat v) = tSucc (qNat v')) by now eapply dredalg_det; eauto using dnf, dnf_qNat.
+  assert (v = v'); [apply qNat_inj; congruence|subst v'].
+  exists (S k); apply murec_intro; tea.
++ intros; now eapply escapeEqTerm.
++ now eapply escapeEqTerm.
+Qed.
+
+Lemma reify_Red_EvalStep {Γ l t t₀ u k v} (rNat : [Γ ||-<l> tNat]) :
+  [t ⇶* t₀] -> dnf t₀ -> closed0 t₀ ->
+  (forall k' : nat, k' < k -> [rNat | Γ ||- qRun t u k' ≅ tZero : tNat]) ->
+  [rNat | Γ ||- qRun t u k ≅ tSucc (qNat v) : tNat] ->
+  [SimpleArr.ArrRedTy rNat rNat | Γ ||- t : tPNat] ->
+  EvalStep Γ t u k v.
+Proof.
+intros.
+assert (rv : [rNat | Γ ||- tApp t (qNat u) : tNat]).
+{ unshelve eapply (SimpleArr.simple_appTerm (F := tNat)); tea; apply qNatRed. }
+assert (Hnfv := rv); apply nf_eval in Hnfv.
+destruct Hnfv as (v₀&Hred&?&?).
+assert (∑ m₀, v₀ = qNat m₀ ×  [rNat | Γ ||- tApp t (qNat u) ≅ qNat m₀ : tNat]) as (m₀&?&?); [|subst v₀].
+{ eapply dnf_closed_qNat; tea.
+  eapply (dred_tApp_qNat_closed0 t t₀ u); eauto. }
+now eapply reify_red_EvalStep.
+Qed.
+
+Lemma StepEvalRedEq : forall Γ l t t₀ u k v (rNat : [Γ ||-<l> tNat]) (rNatNat := SimpleArr.ArrRedTy rNat rNat),
+  [Γ |- t ≅ t₀ : tPNat] -> [t ⇶* t₀] -> dnf t₀ -> closed0 t₀ -> eqnf t t₀ ->
+  [Γ ||-<l> t : arr tNat tNat | rNatNat ] ->
+  (forall k', k' < k -> [rNat | Γ ||- qRun t u k' ≅ tZero : tNat]) ->
+  [rNat | Γ ||- qRun t u k ≅ tSucc (qNat v) : tNat] ->
+  [Γ ||-<l> run model : arr tNat (arr tNat tPNat) | SimpleArr.ArrRedTy rNat (SimpleArr.ArrRedTy rNat rNatNat)] ->
+  [rNat | Γ ||- tStep t (qNat u) ≅ qNat k : tNat].
+Proof.
+intros * Ht Hr Hnf Hc Hannot rt rnil rval rrun.
+assert (rΓ : [|- Γ]) by now eapply wfc_wft, escape.
+eapply redSubstTerm; [eapply qNatRed|].
+transitivity (tStep t₀ (qNat u)).
++ apply redtm_step; eauto using convtm_qNat, dnf_qNat.
+  - now eapply escapeTerm.
+  - reflexivity.
++ assert (EvalStep Γ t u k v).
+  { unshelve eapply reify_Red_EvalStep; tea. }
+  assert (EvalStep Γ t₀ u k v) by now eapply eqnf_EvalStep.
+  eapply redtm_evalstep; tea.
+  - now eapply urefl.
+  - now eapply escapeTerm.
+Qed.
+
+End StepRed.
+
+Section ReflectRed.
+
+Context `{GenericTypingProperties}.
+Context {SN : SNTypingProperties ta _ _ _ _ _}.
+
+Lemma TotalURedEq {Γ l t t' u u'} (rΓ : [|- Γ]) (rU : [Γ ||-<one> U]) (rNat := natRed rΓ) (rNatNat := SimpleArr.ArrRedTy rNat rNat) :
+  [Γ ||-<l> t ≅ t' : arr tNat tNat | rNatNat ] ->
+  [Γ ||-<l> u ≅ u' : tNat | rNat ] ->
+  [Γ ||-<l> run model : arr tNat (arr tNat tPNat) | SimpleArr.ArrRedTy rNat (SimpleArr.ArrRedTy rNat rNatNat)] ->
+  [rU | Γ ||- tTotal t u ≅ tTotal t' u' : U].
+Proof.
+intros rt ru rrun.
+unfold tTotal.
+assert (rNN : [Γ ||-< l > arr tNat (arr tNat tNat)]) by now apply SimpleArr.ArrRedTy.
+assert (rNNN : [Γ ||-< l > arr tNat (arr tNat (arr tNat tNat))]) by now apply SimpleArr.ArrRedTy.
+assert [rNat | Γ ||- u : tNat] by now eapply LRTmEqRed_l.
+assert [rNat | Γ ||- u' : tNat] by now eapply LRTmEqRed_r.
+unshelve eapply tEvalURedEq; tea.
++ unshelve eapply (SimpleArr.simple_appcongTerm (F := tNat)); tea.
+  unshelve eapply (SimpleArr.simple_appcongTerm (F := tNat)); tea.
+  - apply reflLRTmEq; irrelevance0; [reflexivity|]; tea.
+  - eapply QuoteRed, escapeEqTerm.
+    eapply transEqTerm; [|apply LRTmEqSym]; tea.
+  - eapply QuoteRed, escapeEqTerm.
+    eapply transEqTerm; [apply LRTmEqSym|]; tea.
+  - now eapply QuoteRedEq, escapeEqTerm.
++ now eapply StepRedEq.
++ unshelve eapply (SimpleArr.simple_appcongTerm (F := tNat)); tea.
+Qed.
+
+Lemma TotalURed {Γ l t u} (rΓ : [|- Γ]) (rU : [Γ ||-<one> U]) (rNat := natRed rΓ) (rNatNat := SimpleArr.ArrRedTy rNat rNat) :
+  [Γ ||-<l> t : arr tNat tNat | rNatNat ] ->
+  [Γ ||-<l> u : tNat | rNat ] ->
+  [Γ ||-<l> run model : arr tNat (arr tNat tPNat) | SimpleArr.ArrRedTy rNat (SimpleArr.ArrRedTy rNat rNatNat)] ->
+  [rU | Γ ||- tTotal t u : U].
+Proof.
+intros.
+eapply LRTmEqRed_l, TotalURedEq.
++ now eapply reflLRTmEq.
++ now eapply reflLRTmEq.
++ tea.
+Qed.
+
+Lemma TotalRed {Γ l t u} (rΓ : [|- Γ]) (rNat := natRed rΓ) (rNatNat := SimpleArr.ArrRedTy rNat rNat) :
+  [Γ ||-<l> t : arr tNat tNat | rNatNat ] ->
+  [Γ ||-<l> u : tNat | rNat ] ->
+  [Γ ||-<l> run model : arr tNat (arr tNat tPNat) | SimpleArr.ArrRedTy rNat (SimpleArr.ArrRedTy rNat rNatNat)] ->
+  [Γ ||-<one> tTotal t u].
+Proof.
+intros.
+now eapply ElURed, TotalURed.
+Unshelve.
+now eapply LRU_, redUOne.
+Qed.
+
+Fixpoint nShift (n : nat) t := match n with
+| 0 => t
+| S n => tShift (nShift n t)
+end.
+
+Lemma nShiftRed {Γ l n t} (rNatNat : [Γ ||-<l> tPNat]) :
+  [rNatNat | Γ ||- t : tPNat] ->
+  [rNatNat | Γ ||- nShift n t : tPNat].
+Proof.
+revert t; induction n; intros t rt; cbn; tea.
+now apply tShiftRed.
+Qed.
+
+Lemma nShiftAppRedEq {Γ l n m t} (rNat : [Γ ||-<l> tNat]) (rNatNat := SimpleArr.ArrRedTy rNat rNat) :
+  [rNatNat | Γ ||- t : tPNat] ->
+  [rNat | Γ ||- tApp (nShift n t) (qNat m) ≅ tApp t (qNat (n + m)) : tNat].
+Proof.
+intros rt.
+assert (rΓ : [|- Γ]) by now eapply wfc_wft, escape.
+unshelve (irrelevance0; [reflexivity|]); [|now apply (natRed (l := l))|].
+revert m t rt.
+induction n; cbn [nShift plus]; intros.
++ unshelve eapply reflLRTmEq, (SimpleArr.simple_appTerm (F := tNat)); eauto using qNatRed.
++ eapply transEqTerm; [eapply tShiftAppRedEq|].
+  - eapply nShiftRed.
+    now unshelve (irrelevance0; [reflexivity|]).
+  - now apply qNatRed.
+  - cbn [qNat].
+    assert (Hr := IHn (S m) t rt).
+    now replace (n + S m) with (S (n + m)) in Hr by Lia.lia.
+Qed.
+
+Lemma qEvalTyEvalStepRedEq {Γ l t n k v} (rΓ : [|- Γ]) (rU : [Γ ||-<one> U]) (rNat := natRed rΓ) (rNatNat := SimpleArr.ArrRedTy rNat rNat)
+  (f := (tApp (tApp (run model) (qNat (quote model (erase t)))) (qNat n))) :
+  [Γ ||-<l> f : tPNat | rNatNat] ->
+  EvalStep Γ t n k v ->
+  [rU | Γ ||- tEval f (qNat k) (qNat v) ≅ qEvalTy k v : U].
+Proof.
+intros rrun.
+change f with (nShift 0 f).
+change (EvalStep Γ t n k v) with (EvalStep Γ t n (0 + k) v).
+generalize 0 as acc.
+induction k; intros acc Hstep.
++ eapply transEqTerm; [unshelve eapply (tEvalZeroRedEq (l := l))|]; tea.
+  - now apply nShiftRed.
+  - apply qNatRed.
+  - unshelve eapply tIsValRedEq; eauto using qNatRedEq.
+    eapply transEqTerm; [eapply (nShiftAppRedEq (m := 0))|]; tea.
+    eapply dnf_closed_qNatRedEq with (n := S v); [now unshelve eauto using SimpleArr.simple_appTerm, qNatRed|].
+    destruct Hstep as [[k₀ Hk] _ _].
+    apply murec_elim_Some in Hk.
+    now apply run_spec_Some.
++ cbn [qNat].
+  eapply transEqTerm; [unshelve eapply (tEvalSuccRedEq (l := l))|]; eauto using qNatRed.
+  - now apply nShiftRed.
+  - unshelve eapply tEvalURed; unshelve eauto using qNatRed.
+    now unshelve apply tShiftRed, nShiftRed.
+  - cbn [qEvalTy]; apply tAndURedEq; tea.
+    { unshelve eapply tIsNilRedEq; tea.
+      eapply transEqTerm; [eapply (nShiftAppRedEq (m := k))|]; tea.
+      eapply dnf_closed_qNatRedEq with (n := 0); [now unshelve eauto using SimpleArr.simple_appTerm, qNatRed|].
+      destruct Hstep as [[k₀ Hk] _ _].
+      apply (murec_elim_None (k' := (acc + k))) in Hk; [|Lia.lia].
+      now apply run_spec_None.
+    }
+    { apply (IHk (S acc)).
+      now replace (S acc + k) with (acc + S k) by Lia.lia. }
+Qed.
+
+Lemma ReflectRedEq : forall Γ l t t' u u' (rΓ : [|- Γ]) (rNat := natRed rΓ) (rNatNat := SimpleArr.ArrRedTy rNat rNat)
+  (rTotal : [Γ ||-<l> tTotal t u]),
+  [Γ ||-<l> t ≅ t' : arr tNat tNat | rNatNat ] ->
+  [Γ ||-<l> u ≅ u' : tNat | rNat ] ->
+  [Γ ||-<l> run model : arr tNat (arr tNat tPNat) | SimpleArr.ArrRedTy rNat (SimpleArr.ArrRedTy rNat rNatNat)] ->
+  [Γ ||-<l> tReflect t u ≅ tReflect t' u' : tTotal t u | rTotal ].
+Proof.
+intros * rtt' ruu' rrun.
+assert (rt : [Γ ||-<l> t : arr tNat tNat | rNatNat ]) by now eapply LRTmEqRed_l.
+assert (rt' : [Γ ||-<l> t' : arr tNat tNat | rNatNat ]) by now eapply LRTmEqRed_r.
+assert (ru : [Γ ||-<l> u : tNat | rNat ]) by now eapply LRTmEqRed_l.
+assert (ru' : [Γ ||-<l> u' : tNat | rNat ]) by now eapply LRTmEqRed_r.
+assert (rU : [Γ ||-<one> U]) by now apply LRU_, redUOne.
+assert [Γ |- run model : arr tNat (arr tNat (arr tNat tNat))] by now eapply escapeTerm.
+assert [Γ |- tTotal t u ≅ tTotal t' u' : U].
+{ now unshelve eapply escapeEqTerm, TotalURedEq. }
+assert (Hnft := rtt'); apply escapeEqTerm, snty_nf in Hnft.
+assert (Hnfu := ruu'); apply escapeEqTerm, snty_nf in Hnfu.
+destruct Hnft as (t₀&t'₀&[]&[]&?&?&?).
+destruct Hnfu as (u₀&u'₀&[]&[]&?&?&?).
+remember (is_closedn 0 t₀) as ct eqn:Hct; symmetry in Hct.
+assert (Hct' : is_closedn 0 t'₀ = ct).
+{ erewrite eqnf_is_closedn; [tea|now apply Symmetric_eqnf]. }
+remember (is_closedn 0 u₀) as cu eqn:Hcu; symmetry in Hcu.
+assert (Hcu' : is_closedn 0 u'₀ = cu).
+{ erewrite eqnf_is_closedn; [tea|now apply Symmetric_eqnf]. }
+remember (andb ct cu) as cb eqn:Hcb; symmetry in Hcb; destruct cb.
++ destruct ct; [|cbn in Hcb; congruence].
+  destruct cu; [|cbn in Hcb; congruence].
+  clear Hcb.
+
+  assert (∑ n₀, u₀ = qNat n₀ ×  [rNat | Γ ||- u ≅ qNat n₀ : tNat]) as (n₀&?&?) by now eapply dnf_closed_qNat.
+  assert (∑ n'₀, u'₀ = qNat n'₀ ×  [rNat | Γ ||- u' ≅ qNat n'₀ : tNat]) as (n'₀&?&?) by now eapply dnf_closed_qNat.
+  subst.
+  assert (n₀ = n'₀); [|subst n'₀].
+  { eapply red_qNat_inj, transEqTerm, transEqTerm; [now apply LRTmEqSym| |tea]; tea. }
+
+  assert (rvv' : [rNat | Γ ||- tApp t (qNat n₀) ≅ tApp t' (qNat n₀) : tNat]).
+  { unshelve eapply (SimpleArr.simple_appcongTerm (F := tNat)); tea; first [apply qNatRed|apply qNatRedEq]. }
+
+  assert (Hnfv := rvv'); apply escapeEqTerm, snty_nf in Hnfv.
+  destruct Hnfv as (v₀&v'₀&[]&[]&?&?&?).
+
+  assert (rv : [rNat | Γ ||- tApp t (qNat n₀) : tNat]) by now eapply LRTmEqRed_l.
+  assert (rv' : [rNat | Γ ||- tApp t' (qNat n₀) : tNat]) by now eapply LRTmEqRed_r.
+
+
+  assert (∑ m₀, v₀ = qNat m₀ ×  [rNat | Γ ||- tApp t (qNat n₀) ≅ qNat m₀ : tNat]) as (m₀&?&?).
+  { eapply dnf_closed_qNat; tea.
+    eapply (dred_tApp_qNat_closed0 t t₀ n₀); eauto. }
+  assert (∑ m₀, v'₀ = qNat m₀ ×  [rNat | Γ ||- tApp t' (qNat n₀) ≅ qNat m₀ : tNat]) as (m'₀&?&?).
+  { eapply dnf_closed_qNat; tea.
+    eapply (dred_tApp_qNat_closed0 t' t'₀ n₀); eauto. }
+  subst.
+
+  subst.
+  let H := match goal with H : eqnf (qNat _) (qNat _) |- _ => H end in
+  unfold eqnf in H; rewrite !erase_qNat in H; apply qNat_inj in H; subst m'₀.
+
+  assert (forall k : nat, [rNat | Γ ||- qRun t₀ n₀ k : tNat]).
+  { intros k; unfold qRun.
+    unshelve eapply (SimpleArr.simple_appTerm (F := tNat)); tea; [|apply qNatRed].
+    assert (rT : [Γ ||-< l > arr tNat (arr tNat tNat)]) by now apply SimpleArr.ArrRedTy.
+    unshelve eapply (SimpleArr.simple_appTerm (F := tNat)); tea; [|apply qNatRed].
+    unshelve eapply (SimpleArr.simple_appTerm (F := tNat)); tea; apply qNatRed.
+  }
+
+  assert (∑ k, EvalStep Γ t₀ n₀ k m₀) as [k Hk].
+  { eapply reify_EvalStep; [tea|].
+    now eapply dred_tApp_qNat_compat. }
+
+  assert [rNat | Γ ||- tQuote t ≅ qNat (model.(quote) (erase t₀)) : tNat].
+  { eapply redSubstTerm; [now eapply qNatRed|].
+    transitivity (tQuote t₀).
+    - now eapply redtm_quote.
+    - eapply redtm_evalquote; tea; now eapply urefl. }
+
+  assert [rNat | Γ ||- tStep t u ≅ qNat k : tNat].
+  { eapply redSubstTerm; [now eapply qNatRed|].
+    transitivity (tStep t₀ (qNat n₀)).
+    - now eapply redtm_step.
+    - eapply redtm_evalstep; tea; now eapply urefl. }
+
+  assert [rNat | Γ ||- tApp t u ≅ qNat m₀ : tNat].
+  { eapply (transEqTerm (u := tApp t (qNat n₀))); [|tea].
+    unshelve eapply (SimpleArr.simple_appcongTerm (F := tNat)); tea; [|apply qNatRed].
+    now eapply reflLRTmEq. }
+
+  assert [rNatNat | Γ ||- tApp (tApp (run model) (tQuote t)) u ≅
+    tApp (tApp (run model) (qNat (model.(quote) (erase t₀)))) (qNat n₀) : tPNat].
+  { unshelve eapply (SimpleArr.simple_appcongTerm (F := tNat)); eauto using SimpleArr.ArrRedTy, qNatRed.
+    unshelve eapply (SimpleArr.simple_appcongTerm (F := tNat)); eauto using SimpleArr.ArrRedTy, qNatRed, LRTmEqRed_l, LRTmEqRed_r.
+    now eapply reflLRTmEq. }
+
+  assert [rU | Γ ||- tTotal t u ≅ qEvalTy k m₀ : U].
+  { unfold tTotal; eapply transEqTerm.
+    + eapply tEvalURedEq; tea.
+    + eapply qEvalTyEvalStepRedEq; [|tea].
+      now eapply LRTmEqRed_r. }
+
+  assert [Γ |- tTotal t u ≅ tTotal t (qNat n₀)].
+  { unshelve eapply convty_term, escapeEqTerm; [|exact rU|].
+    eapply TotalURedEq; [now eapply reflLRTmEq|tea|tea]. }
+
+  assert [Γ |- tTotal t' u' ≅ tTotal t' (qNat n₀)].
+  { unshelve eapply convty_term, escapeEqTerm; [|exact rU|].
+    eapply TotalURedEq; [now eapply reflLRTmEq|tea|tea]. }
+
+  eapply (red_redtm_exp (t := qEvalTm k m₀) (u := qEvalTm k m₀)).
+  - etransitivity; [now eapply redtm_reflect|].
+    eapply redtm_conv; [|now symmetry].
+    now eapply redtm_evalreflect.
+  - eapply redtm_conv; [|symmetry; now apply convty_term].
+    etransitivity; [now eapply redtm_reflect|].
+    eapply redtm_conv; [|now symmetry].
+    eapply redtm_evalreflect; tea.
+    now eapply eqnf_EvalStep.
+  - unshelve eapply LRTmEqRedConv, reflLRTmEq, qEvalTmRed; tea.
+    unshelve eapply ElURedEq, LRTmEqSym; tea.
+    irrelevance0; [reflexivity|]; tea.
++ eapply neuTermEqRed.
+  - eapply redtm_reflect; tea.
+    all: now eapply escapeTerm.
+  - eapply redtm_conv; [eapply redtm_reflect|]; tea.
+    symmetry; now apply convty_term.
+  - apply ty_reflect; first [now symmetry|now eapply escapeTerm].
+  - apply ty_reflect; [..|now eapply escapeTerm].
+    * symmetry; transitivity t'; [now eapply escapeEqTerm|tea].
+    * symmetry; transitivity u'; [now eapply escapeEqTerm|tea].
+  - eapply convneu_reflect; tea.
+    * etransitivity; [now symmetry|].
+      etransitivity; [now eapply escapeEqTerm|tea].
+    * etransitivity; [now symmetry|].
+      etransitivity; [now eapply escapeEqTerm|tea].
+    * now symmetry.
+    * now symmetry.
+    * rewrite Hct, Hcu; destruct ct, cu; compute; now eauto.
+    * rewrite Hct', Hcu'; destruct ct, cu; compute; now eauto.
+Qed.
+
+Lemma ReflectRed : forall Γ l t u (rΓ : [|- Γ])
+  (rNat := natRed rΓ) (rNatNat := SimpleArr.ArrRedTy rNat rNat)
+  (rTotal : [Γ ||-<l> tTotal t u]),
+  [Γ ||-<l> t : arr tNat tNat | rNatNat] ->
+  [Γ ||-<l> u : tNat | rNat] ->
+  [Γ ||-<l> run model : arr tNat (arr tNat tPNat) | SimpleArr.ArrRedTy rNat (SimpleArr.ArrRedTy rNat rNatNat)] ->
+  [Γ ||-<l> tReflect t u : tTotal t u | rTotal].
+Proof.
+intros.
+eapply LRTmEqRed_l, ReflectRedEq; tea.
++ now eapply reflLRTmEq.
++ now eapply reflLRTmEq.
+Qed.
+
+Lemma qTmEvalRed {Γ l t t₀ u k v} (rΓ : [|-Γ]) (rNat := natRed (l := l) rΓ) (rNatNat := SimpleArr.ArrRedTy rNat rNat)
+  (rTotal : [Γ ||-<one> tTotal t (qNat u)]) :
+  [Γ |- t ≅ t₀ : tPNat] -> [t ⇶* t₀] -> dnf t₀ -> closed0 t -> eqnf t t₀ ->
+  [Γ ||-<l> run model : arr tNat (arr tNat tPNat) | SimpleArr.ArrRedTy rNat (SimpleArr.ArrRedTy rNat rNatNat)] ->
+  [rNatNat | Γ ||- t : tPNat] ->
+  (forall k', k' < k -> [rNat | Γ ||- qRun t u k' ≅ tZero : tNat]) ->
+  [rNat | Γ ||- qRun t u k ≅ tSucc (qNat v) : tNat] ->
+  [rTotal | Γ ||- qEvalTm k v : tTotal t (qNat u)].
+Proof.
+intros ?? Hnf Hc Heq rrun rt rnil rval.
+unshelve epose (rU := LRU_ (redUOne _)); [|tea|].
+assert (rapp : [rNat | Γ ||- tApp t (qNat u) : tNat]).
+{ unshelve eapply (SimpleArr.simple_appTerm (F := tNat)), qNatRed; tea. }
+assert (Hred : ∑ v, [tApp t (qNat u) ⇶* qNat v]).
+{ assert (rapp' := rapp).
+  apply nf_eval in rapp'.
+  destruct rapp' as (v'&?&?&?).
+  assert (closed0 v').
+  { eapply dredalg_closed0; [tea|unfold closed0; cbn].
+    apply andb_true_intro; split; [tea|apply closedn_qNat]. }
+  unshelve eapply dnf_closed_qNat in rapp; [| |tea| |]; tea.
+  destruct rapp as (n&?&?); subst.
+  now exists n. }
+destruct Hred as [v' Hred].
+assert (Hev : EvalStep Γ t u k v).
+{ eapply reify_red_EvalStep.
+  + intros; now unshelve apply rnil.
+  + now unshelve eapply rval.
+  + Unshelve. all: tea. }
+assert (v' = v); [|subst v'].
+{ destruct Hev as [[? Hev]].
+  apply murec_elim_Some, eval_dredalg in Hev.
+  apply dred_erase_qNat_compat in Hred; cbn in Hred.
+  rewrite erase_qNat in Hred.
+  eapply qNat_inj, dredalg_det; eauto using dnf_qNat. }
+assert [rNat | Γ ||- tQuote t ≅ qNat (model.(quote) (erase t)) : tNat].
+{ eapply QuoteEvalRedEq; tea.
+  now eapply dredalg_closed0. }
+assert (rEqLU : [rU | Γ ||- (tTotal t (qNat u)) ≅
+  tEval (tApp (tApp (run model) (qNat (quote model (erase t)))) (qNat u)) (qNat k) (qNat v) : U]).
+{ unshelve eapply tEvalURedEq; tea.
+  + unshelve eapply simple_AppRedEq, qNatRedEq; eauto using SimpleArr.ArrRedTy; try apply qNatRed.
+    unshelve eapply simple_AppRedEq; [..|tea].
+    now apply reflLRTmEq.
+  + eapply StepEvalRedEq with (v := v); tea.
+    now eapply dredalg_closed0.
+  + eapply dnf_closed_qNatRedEq; tea.
+}
+assert (rEqRU : [rU | Γ ||- tEval (tApp (tApp (run model) (qNat (quote model (erase t)))) (qNat u)) (qNat k) (qNat v)
+  ≅ qEvalTy k v : U]).
+{ unshelve eapply qEvalTyEvalStepRedEq; tea.
+  unshelve eapply SimpleArr.simple_appTerm, qNatRed; eauto using SimpleArr.ArrRedTy.
+  unshelve eapply SimpleArr.simple_appTerm, qNatRed; eauto using SimpleArr.ArrRedTy. }
+assert (rEqU : [rU | Γ ||- (tTotal t (qNat u)) ≅ qEvalTy k v : U]).
+{ now eapply transEqTerm. }
+assert (rEvalTy : [Γ ||-<one> qEvalTy k v]).
+{ unshelve eapply ElURed, LRTmEqRed_r, rEqU. }
+assert (rEq : [rEvalTy | Γ ||- qEvalTy k v ≅ (tTotal t (qNat u))]) .
+{ now unshelve eapply ElURedEq, LRTmEqSym. }
+eapply LRTmRedConv; [eapply LRTyEqIrrelevantCum, rEq|].
+irrelevance0; [reflexivity|]; now unshelve eapply qEvalTmRed.
+Unshelve.
+{ exact one. }
+{ apply (LRCumulative rEvalTy). }
+Qed.
+
+Lemma ReflectEvalRedEq : forall Γ l t t₀ u k v (rΓ : [|- Γ])
+  (rNat := natRed (l := l) rΓ) (rNatNat := SimpleArr.ArrRedTy rNat rNat)
+  (rTotal : [Γ ||-<one> tTotal t (qNat u)]),
+  [Γ |- t ≅ t₀ : tPNat] -> [t ⇶* t₀] -> dnf t₀ -> closed0 t -> eqnf t t₀ ->
+  [Γ ||-<l> t : arr tNat tNat | rNatNat ] ->
+  (forall k', k' < k -> [rNat | Γ ||- qRun t u k' ≅ tZero : tNat]) ->
+  [rNat | Γ ||- qRun t u k ≅ tSucc (qNat v) : tNat] ->
+  [Γ ||-<l> run model : arr tNat (arr tNat tPNat) | SimpleArr.ArrRedTy rNat (SimpleArr.ArrRedTy rNat rNatNat)] ->
+  [rTotal | Γ ||- tReflect t (qNat u) ≅ qEvalTm k v : tTotal t (qNat u)].
+Proof.
+intros * ????? rt rnil rval rrun.
+eapply redSubstTerm.
++ eapply qTmEvalRed; tea.
++ assert [Γ |-[ ta ] run model : arr tNat (arr tNat tPNat)] by now eapply escapeTerm.
+  assert (closed0 t₀) by now eapply dredalg_closed0.
+  transitivity (tReflect t₀ (qNat u)).
+  - apply redtm_reflect; eauto using dnf_qNat, convtm_qNat, @RedClosureAlg.
+  - apply redtm_evalreflect; tea.
+    eapply eqnf_EvalStep; [tea|].
+    eapply reify_Red_EvalStep; tea.
+Qed.
+
+End ReflectRed.
+
+Section Valid.
+
+Context `{GenericTypingProperties}.
+
+Lemma mkValid {Γ l A t} (vΓ : [||-v Γ]) (vA : [Γ ||-v< l > A | vΓ]) :
+  (forall Δ σ σ' (wfΔ : [ |- Δ]) (Vσ : [vΓ | Δ ||-v σ : Γ | wfΔ]),
+    [vΓ | Δ ||-v σ' : Γ | wfΔ] ->
+    [vΓ | Δ ||-v σ ≅ σ' : Γ | wfΔ | Vσ] ->
+    [validTy vA wfΔ Vσ | Δ ||- t[σ] ≅ t[σ'] : A[σ]]) ->
+  [Γ ||-v< l > t : A | vΓ | vA].
+Proof.
+intros vt; split; [|tea].
+intros; eapply LRTmEqRed_l.
+apply vt; tea.
+now apply reflSubst.
+Qed.
+
+End Valid.
+
+Section ReflectValid.
+
+Context `{GenericTypingProperties}.
+Context {SN : SNTypingProperties ta _ _ _ _ _}.
 
 Definition evalValid {Γ l t k r} (vΓ : [||-v Γ])
   (vNat := natValid (l := l) vΓ)
@@ -753,7 +1677,7 @@ Proof.
 assert (vEval : forall Δ σ (vΔ : [|- Δ]) (vσ : [vΓ | Δ ||-v σ : Γ | vΔ]),
   [Δ ||-< one > tEval t[σ] k[σ] r[σ]]).
 { intros Δ σ vΔ **.
-  unshelve eapply tEvalRedTy; tea.
+  unshelve eapply tEvalRed; tea.
   - destruct vt as [vt _].
     irrelevance0; [reflexivity|]; now unshelve apply vt.
   - destruct vk as [vk _].
@@ -775,7 +1699,7 @@ unshelve econstructor.
     * shelve.
     * refine (embRedTyOne relL).
     * apply relEq. }
-  unshelve eapply tEvalRedEq.
+  unshelve eapply tEvalURedEq.
   - shelve.
   - now unshelve apply natRed.
   - now unshelve (apply SimpleArr.ArrRedTy; apply natRed).
@@ -789,167 +1713,7 @@ unshelve econstructor.
   Unshelve. all: tea.
 Qed.
 
-End Utils.
-
-Section ReflectRed.
-
-Context `{GenericTypingProperties}.
-Context {SN : SNTypingProperties ta _ _ _ _ _}.
-
-(*
-Lemma ReflectRed : forall Γ l t u (rΓ : [|- Γ])
-  (rNat := natRed rΓ) (rNatNat := SimpleArr.ArrRedTy rNat rNat)
-  (rTotal : [Γ ||-<l> tTotal t u]),
-  [Γ ||-<l> t : arr tNat tNat | rNatNat] ->
-  [Γ ||-<l> u : tNat | rNat] ->
-  [Γ ||-<l> run model : arr tNat (arr tNat tPNat) | SimpleArr.ArrRedTy rNat (SimpleArr.ArrRedTy rNat rNatNat)] ->
-  [Γ ||-<l> tReflect t u : tTotal t u | rTotal].
-Proof.
-intros * rt ru rrun.
-pose (rTotal' := normRedΣ0 (Induction.invLRΣ rTotal)); refold.
-fold (tTotal t u) in rTotal'.
-eapply LRTmRedIrrelevant' with (lrA := LRSig' rTotal'); [reflexivity|].
-destruct (nf_eval rt) as [r [Hrnf [Hr Hrconv]]].
-destruct (nf_eval ru) as [n [Hnnf [Hn Hnconv]]].
-remember (is_closedn 0 r) as cr eqn:Hcr; symmetry in Hcr.
-remember (is_closedn 0 n) as cn eqn:Hcn; symmetry in Hcn.
-remember (andb cr cn) as cb eqn:Hcb; symmetry in Hcb; destruct cb.
-+ destruct cr; [|cbn in Hcb; congruence].
-  destruct cn; [|cbn in Hcb; congruence].
-  assert (∑ n₀, n = qNat n₀) as [n₀]; [|subst].
-  { eapply dnf_closed_qNat; [apply ru| | |]; tea. }
-  clear Hcb Hn Hcn.
-  assert (rapp : [rNat | _ ||- tApp t u : tNat]).
-  { eapply SimpleArr.simple_appTerm; tea. }
-  assert (Heval : ∑ m k, eval true (tApp (erase t) u) k = Some (qNat m)).
-  { admit. }
-  destruct Heval as (m&k&Heval).
-(*   eapply (redSubstTerm (u := qTotal (model.(quote) (erase r)) n₀ k m)). *)
-(*
-  eapply LRTmRedConv.
-(*   - cbn; unfold qTotal. *)
-(*   unshelve eexists (qTotal (model.(quote) (erase r)) n₀ k m) _. *)
-admit.
-  - intros; unshelve irrelevance0; [exact l| |now apply natRed|reflexivity|].
-    eexists (qNat k); [|now apply convtm_qNat|now apply qNatRed].
-    split; [now apply ty_qNat|].
-    unfold ren1, Ren1_well_wk; rewrite qTotal_ren.
-    apply redtm_fst_beta.
-    * gen_typing.
-    * admit.
-    * now apply ty_qNat.
-    * rewrite tEval_subst; cbn; rewrite run_subst, quote_subst, !qNat_subst, erase_is_closed0_subst_id; tea.
-      admit.
-  - admit.
-  - admit.
-  - admit.
-  - admit.
-*)
-admit.
-+ assert ([Γ |-[ ta ] run model : arr tNat (arr tNat tPNat)]).
-  { unshelve eapply escapeTerm; tea. }
-(*
-  assert [Γ |- tTotal r n ≅ tTotal t u].
-  { eapply convty_term, tTotal_cong.
-    + admit.
-    + admit.
-  }
-*)
-  eapply redSubstTerm; [|eapply redtm_reflect; tea]; try now eapply escapeTerm.
-  apply neuTerm.
-  - eapply ty_conv; [eapply ty_reflect; first [now eapply urefl|tea]|tea].
-    eapply convty_term, tTotal_cong.
-    admit.
-    admit.
-  - assert ((~ is_true (is_closedn 0 r)) + (~ is_true (is_closedn 0 n))).
-    { destruct (is_closedn 0 r); [|left; congruence].
-      destruct (is_closedn 0 n); [|right; congruence].
-      subst; cbn in Hcb; congruence. }
-    eapply convneu_reflect; first [now eapply urefl|now symmetry|tea].
-Admitted.
-*)
-
-Lemma neuTermEqRed {Γ l A t t' n n'} (RA : [Γ ||-<l> A]) :
-  [Γ |- t ⤳* n : A] ->
-  [Γ |- t' ⤳* n' : A] ->
-  [Γ |- n : A] -> [Γ |- n' : A] -> [Γ |- n ~ n' : A] -> [Γ ||-<l> t ≅ t' : A | RA].
-Proof.
-intros Ht Ht' Hn Hn' Hnn'.
-eapply transEqTerm; [|eapply LRTmEqSym, transEqTerm]; [| |eapply LRTmEqSym, neuTermEq]; [..|tea]; tea.
-- eapply redSubstTerm; [|tea]; try now eapply escapeTerm.
-  eapply neuTerm; [tea|now eapply lrefl].
-- eapply redSubstTerm; [|tea]; try now eapply escapeTerm.
-  eapply neuTerm; [tea|now eapply urefl].
-Qed.
-
-Lemma ReflectRedEq : forall Γ l t t' u u' (rΓ : [|- Γ]) (rNat := natRed rΓ) (rNatNat := SimpleArr.ArrRedTy rNat rNat)
-  (rTotal : [Γ ||-<l> tTotal t u]),
-  [Γ ||-<l> t : arr tNat tNat | rNatNat ] ->
-  [Γ ||-<l> t' : arr tNat tNat | rNatNat ] ->
-  [Γ ||-<l> u : tNat | rNat ] ->
-  [Γ ||-<l> u' : tNat | rNat ] ->
-  [Γ ||-<l> t ≅ t' : arr tNat tNat | rNatNat ] ->
-  [Γ ||-<l> u ≅ u' : tNat | rNat ] ->
-  [Γ ||-<l> run model : arr tNat (arr tNat tPNat) | SimpleArr.ArrRedTy rNat (SimpleArr.ArrRedTy rNat rNatNat)] ->
-  [Γ ||-<l> tReflect t u ≅ tReflect t' u' : tTotal t u | rTotal ].
-Proof.
-intros * rt rt' ru ru' rtt' ruu' rrun.
-(* pose (rTotal' := normRedΣ0 (Induction.invLRΣ rTotal)); refold. *)
-(* fold (tTotal t u) in rTotal'. *)
-(* eapply LRTmEqIrrelevant' with (lrA := LRSig' rTotal'); [reflexivity|]. *)
-assert (Hnft := rtt'); apply escapeEqTerm, snty_nf in Hnft.
-assert (Hnfu := ruu'); apply escapeEqTerm, snty_nf in Hnfu.
-destruct Hnft as (t₀&t'₀&[]&[]&?&?&?).
-destruct Hnfu as (u₀&u'₀&[]&[]&?&?&?).
-remember (is_closedn 0 t₀) as ct eqn:Hct; symmetry in Hct.
-assert (Hct' : is_closedn 0 t'₀ = ct).
-{ erewrite eqnf_is_closedn; [tea|now apply Symmetric_eqnf]. }
-remember (is_closedn 0 u₀) as cu eqn:Hcu; symmetry in Hcu.
-assert (Hcu' : is_closedn 0 u'₀ = cu).
-{ erewrite eqnf_is_closedn; [tea|now apply Symmetric_eqnf]. }
-remember (andb ct cu) as cb eqn:Hcb; symmetry in Hcb; destruct cb.
-+ destruct ct; [|cbn in Hcb; congruence].
-  destruct cu; [|cbn in Hcb; congruence].
-  assert (∑ n₀, u₀ = qNat n₀) as [n₀]; [|subst].
-  { eapply dnf_closed_qNat; [apply ru| | |]; tea. }
-  assert (∑ n'₀, u'₀ = qNat n'₀) as [n'₀]; [|subst].
-  { eapply dnf_closed_qNat; [apply ru'| | |]; tea. }
-  clear Hcu Hcu' Hcb.
-  eapply red_redtm_exp.
-  - admit.
-  - admit.
-  - admit.
-+ eapply neuTermEqRed.
-  - eapply redtm_reflect; tea.
-    all: now eapply escapeTerm.
-  - admit.
-  - admit.
-  - admit.
-  - eapply convneu_reflect.
-Admitted.
-
-Lemma ReflectRed : forall Γ l t u (rΓ : [|- Γ])
-  (rNat := natRed rΓ) (rNatNat := SimpleArr.ArrRedTy rNat rNat)
-  (rTotal : [Γ ||-<l> tTotal t u]),
-  [Γ ||-<l> t : arr tNat tNat | rNatNat] ->
-  [Γ ||-<l> u : tNat | rNat] ->
-  [Γ ||-<l> run model : arr tNat (arr tNat tPNat) | SimpleArr.ArrRedTy rNat (SimpleArr.ArrRedTy rNat rNatNat)] ->
-  [Γ ||-<l> tReflect t u : tTotal t u | rTotal].
-Proof.
-intros.
-eapply LRTmEqRed_l, ReflectRedEq; tea.
-+ now eapply reflLRTmEq.
-+ now eapply reflLRTmEq.
-Qed.
-
-End ReflectRed.
-
-Section ReflectValid.
-
-Context `{GenericTypingProperties}.
-Context {SN : SNTypingProperties ta _ _ _ _ _}.
-
-Lemma TyCumValid@{u i j k l u' i' j' k' l'} l Γ (vΓ : VPack@{u} Γ) A :
+Lemma TyCumValid@{u i j k l u' i' j' k' l'} {l Γ} {vΓ : VPack@{u} Γ} {A} :
 typeValidity@{u i j k l} Γ vΓ l A -> typeValidity@{u' i' j' k' l'} Γ vΓ l A.
 Proof.
 intros [ty eq]; unshelve econstructor.
@@ -958,6 +1722,7 @@ intros [ty eq]; unshelve econstructor.
 + intros.
   now eapply LRTyEqIrrelevantCum, eq.
 Qed.
+
 
 Context {Γ l t u} (vΓ : [||-v Γ])
   (vNat := natValid (l := l) vΓ)
@@ -970,7 +1735,18 @@ Context {Γ l t u} (vΓ : [||-v Γ])
 
 Lemma StepValid : [ Γ ||-v< l > tStep t u : tNat | vΓ | vNat ].
 Proof.
-Admitted.
+eapply mkValid.
+intros Δ σ σ' vΔ vσ vσ' vσσ'.
+cbn - [vNat]; apply StepRedEq.
++ destruct vt as [_ vte].
+  irrelevance0; [reflexivity|]; now eapply vte.
++ destruct vu as [_ vue].
+  irrelevance0; [reflexivity|]; now eapply vue.
++ destruct vrun as [vrun0 ?].
+  rewrite <- (run_subst σ).
+  irrelevance0; [reflexivity|]; now eapply vrun0.
+  Unshelve. all: tea.
+Qed.
 
 Definition totalValid : [Γ ||-v< one > tTotal t u | vΓ].
 Proof.
@@ -981,44 +1757,175 @@ apply (evalValid (l := l)).
   - apply vrun.
   - apply QuoteValid; tea.
   - tea.
-+ admit.
++ apply StepValid.
 + eapply (simple_appValid (F := tNat)); tea.
 Unshelve. all: tea.
 apply simpleArrValid; tea.
-Admitted.
+Qed.
+
+End ReflectValid.
+
+Section ReflectValid.
+
+Context `{GenericTypingProperties}.
+Context {SN : SNTypingProperties ta _ _ _ _ _}.
+
+Context {Γ l t u} (vΓ : [||-v Γ])
+  (vNat := natValid (l := l) vΓ)
+  (vArr := simpleArrValid vΓ vNat vNat)
+  (vRun := simpleArrValid vΓ vNat (simpleArrValid vΓ vNat vArr))
+  (vrun : [ Γ ||-v< l > run model : arr tNat (arr tNat tPNat) | vΓ | vRun ])
+  (vt : [ Γ ||-v< l > t : arr tNat tNat | vΓ | vArr ])
+  (vu : [ Γ ||-v< l > u : tNat | vΓ | vNat ])
+.
+
+Notation totalValid := (TyCumValid (totalValid vΓ vrun vt vu)).
 
 Lemma ReflectValid : [ Γ ||-v< one > tReflect t u : tTotal t u | vΓ | totalValid ].
 Proof.
-split; cbn.
-- intros Δ σ vΔ vσ; instValid vσ.
-  assert (Rtotal : [Δ ||-< one > tTotal t[σ] u[σ]]).
-  { rewrite <- tTotal_subst; eapply (validTy totalValid vΔ vσ). }
-  unshelve irrelevance0; try exact Rtotal; [now rewrite tTotal_subst|].
-  unshelve eapply ReflectRed; tea.
-  + irrelevance0; [reflexivity|]; unshelve eapply vt; tea.
-  + rewrite <- (run_subst σ); irrelevance0; [reflexivity|]; apply Rvrun.
-- intros Δ σ σ' vΔ vσ vσ' vσσ'.
-  assert (Rtotal : [Δ ||-< one > tTotal t[σ] u[σ]]).
-  { rewrite <- tTotal_subst; eapply (validTy totalValid vΔ vσ). }
-  unshelve irrelevance0; try exact Rtotal; [now rewrite tTotal_subst|].
-  eapply ReflectRedEq.
-  + irrelevance0; [reflexivity|]; unshelve eapply vt; tea.
-  + irrelevance0; [reflexivity|]; unshelve eapply vt; tea.
-  + irrelevance0; [reflexivity|]; unshelve eapply vu; tea.
-  + irrelevance0; [reflexivity|]; unshelve eapply vu; tea.
-  + irrelevance0; [reflexivity|]; unshelve eapply vt; tea.
-  + irrelevance0; [reflexivity|]; unshelve eapply vu; tea.
-  + rewrite <- (run_subst σ); irrelevance0; [reflexivity|]; apply vrun.
-  Unshelve. all: tea.
+apply mkValid; intros; cbn.
+pose (rNat := natRed (l := l) wfΔ).
+assert (rrun : [SimpleArr.ArrRedTy (natRed wfΔ)
+   (SimpleArr.ArrRedTy rNat (SimpleArr.ArrRedTy rNat rNat)) | Δ ||- run model : arr tNat (arr tNat (arr tNat tNat))]).
+{ rewrite <- (run_subst σ).
+  unshelve (irrelevance0; [|apply vrun]); eauto. }
+unshelve (irrelevance0; [symmetry; apply tTotal_subst|]); [exact one| |].
++ unshelve eapply LRCumulative, TotalRed; tea.
+  - eapply LRTmRedIrrelevant' with (A := (arr tNat tNat)[σ]); [|unshelve eapply vt]; tea.
+    reflexivity. 
+  - irrelevance0; [reflexivity|unshelve eapply vu]; tea.
++ unshelve (irrelevance0; [reflexivity|]); [|unshelve eapply TotalRed|unshelve eapply ReflectRedEq]; tea.
+  - eapply LRTmRedIrrelevantCum'; [reflexivity|].
+    now unshelve apply vt.
+  - eapply LRTmRedIrrelevantCum'; [reflexivity|].
+    now unshelve apply vu.
+  - eapply LRTmRedIrrelevantCum'; [reflexivity|].
+    apply rrun.
+  - eapply LRTmEqIrrelevantCum'; [reflexivity|].
+    now apply vt.
+  - eapply LRTmEqIrrelevantCum'; [reflexivity|].
+    now apply vu.
+  - eapply LRTmRedIrrelevantCum'; [reflexivity|].
+    apply rrun.
+Qed.
+
+End ReflectValid.
+
+Section StepEvalValid.
+
+Context `{GenericTypingProperties}.
+Context {SN : SNTypingProperties ta _ _ _ _ _}.
+
+Context {Γ l t} {u k v : nat} (vΓ : [||-v Γ])
+  (vNat := natValid (l := l) vΓ)
+  (vArr := simpleArrValid vΓ vNat vNat)
+  (vRun := simpleArrValid vΓ vNat (simpleArrValid vΓ vNat vArr))
+  (vrun : [ Γ ||-v< l > run model : arr tNat (arr tNat tPNat) | vΓ | vRun ])
+  (vt : [ Γ ||-v< l > t : arr tNat tNat | vΓ | vArr ])
+.
+
+Lemma StepEvalValid :
+  dnf t -> closed0 t ->
+  (forall k', k' < k -> [Γ ||-v<l> qRun t u k' ≅ tZero : tNat | vΓ | vNat]) ->
+  [Γ ||-v<l> qRun t u k ≅ tSucc (qNat v) : tNat | vΓ | vNat] ->
+  [Γ ||-v<l> tStep t (qNat u) ≅ qNat k : tNat | vΓ | vNat].
+Proof.
+intros Hnf Hc Hnil Hval; constructor; intros.
+cbn - [LRPack.eqTm validTy]; rewrite !qNat_subst.
+pose (rNat := natRed (l := l) wfΔ).
+assert (rPNat := SimpleArr.ArrRedTy rNat rNat).
+assert (rt : [rPNat | Δ ||- t[σ] : tPNat]).
+{ irrelevance0; [reflexivity|]; now unshelve eapply vt. }
+destruct (nf_eval rt) as (t₀&?&?&?).
+eapply StepEvalRedEq with (v := v); tea.
+- now eapply dredalg_closed0, closed0_subst.
+- now eapply dnf_closed_subst_eqnf.
+- irrelevance0; [reflexivity|].
+  now unshelve apply vt.
+- intros k' Hk'.
+  rewrite <- qRun_subst; tea.
+  now apply Hnil.
+- rewrite <- qRun_subst; tea.
+  rewrite <- qNat_subst with (σ := σ).
+  now apply Hval.
+- rewrite <- (run_subst σ).
+  irrelevance0; [reflexivity|].
+  now unshelve apply vrun.
+Qed.
+
+Context {vTotal : [Γ ||-v< one > tTotal t (qNat u) | vΓ]}.
+
+Lemma qTmEvalValid :
+  dnf t -> closed0 t ->
+  (forall k', k' < k -> [Γ ||-v<l> qRun t u k' ≅ tZero : tNat | vΓ | vNat]) ->
+  [Γ ||-v<l> qRun t u k ≅ tSucc (qNat v) : tNat | vΓ | vNat] ->
+  [Γ ||-v< one > qEvalTm k v : tTotal t (qNat u) | vΓ | vTotal].
+Proof.
+intros Hnf Hc Hnil Hval.
+apply mkValid.
+intros; cbn - [LRPack.eqTm validTy]; rewrite !qEvalTm_subst.
+apply reflLRTmEq.
+pose (rNat := natRed (l := l) wfΔ).
+pose (rNatNat := SimpleArr.ArrRedTy rNat rNat).
+assert (rt : [rNatNat | Δ ||- t[σ] : tPNat]).
+{ eapply LRTmRedIrrelevantCum'; [reflexivity|]; now unshelve eapply vt. }
+assert (rrun : [SimpleArr.ArrRedTy rNat (SimpleArr.ArrRedTy rNat rNatNat) | Δ ||- run model : arr tNat (arr tNat (arr tNat tNat))]).
+{ rewrite <- (run_subst σ).
+  unshelve (irrelevance0; [|apply vrun]); eauto. }
+destruct (nf_eval rt) as (t₀&?&?&?).
+assert (Hrw : tTotal t[σ] (qNat u) = (tTotal t (qNat u))[σ]).
+{ now rewrite tTotal_subst, qNat_subst. }
+unshelve (irrelevance0; [apply Hrw|eapply qTmEvalRed]); tea.
++ unshelve eapply TotalRed; tea.
+  - eapply LRTmRedIrrelevantCum'; [reflexivity|]; now unshelve eapply vt.
+  - eapply qNatRed.
+  - eapply LRTmRedIrrelevantCum'; [reflexivity|]; now unshelve eapply rrun.
++ now apply closed0_subst.
++ now apply dnf_closed_subst_eqnf.
++ rewrite <- (run_subst σ).
+  eapply LRTmRedIrrelevantCum'; [reflexivity|]; now unshelve apply vrun.
++ eapply LRTmRedIrrelevantCum'; [reflexivity|]; now unshelve eapply vt.
++ intros.
+  rewrite <- qRun_subst; tea.
+  now unshelve eapply LRTmEqIrrelevantCum', Hnil.
++ rewrite <- qRun_subst; tea.
+  rewrite <- (qNat_subst _ σ).
+  now unshelve eapply LRTmEqIrrelevantCum', Hval.
 Qed.
 
 Lemma ReflectEvalValid :
-  dnf t -> closed0 t -> dnf u -> closed0 u ->
-  [ Γ ||-v< one > tReflect t u ≅ tZero : tTotal t u | vΓ | totalValid ].
+  dnf t -> closed0 t ->
+  (forall k', k' < k -> [Γ ||-v<l> qRun t u k' ≅ tZero : tNat | vΓ | vNat]) ->
+  [Γ ||-v<l> qRun t u k ≅ tSucc (qNat v) : tNat | vΓ | vNat] ->
+  [Γ ||-v<one> tReflect t (qNat u) ≅ qEvalTm k v : tTotal t (qNat u) | vΓ | vTotal].
 Proof.
-Admitted.
+intros Hnf Hc Hnil Hval; constructor; intros; cbn.
+rewrite qEvalTm_subst, qNat_subst.
+assert (Hrw : tTotal t[σ] (qNat u) = (tTotal t (qNat u))[σ]).
+{ now rewrite tTotal_subst, qNat_subst. }
+pose (rNat := natRed (l := l) wfΔ).
+pose (rNatNat := SimpleArr.ArrRedTy rNat rNat).
+assert (rt : [rNatNat | Δ ||- t[σ] : tPNat]).
+{ eapply LRTmRedIrrelevantCum'; [reflexivity|]; now unshelve eapply vt. }
+destruct (nf_eval rt) as (t₀&?&?&?).
+unshelve (eapply LRTmEqIrrelevantCum'; [exact Hrw|]); [shelve|..].
++ unshelve eapply TotalRed; tea.
+  - eapply qNatRed.
+  - rewrite <- (run_subst σ).
+    eapply LRTmRedIrrelevantCum'; [reflexivity|]; now unshelve eapply vrun.
++ unshelve eapply ReflectEvalRedEq with (t₀ := t₀); tea.
+  - now apply closed0_subst.
+  - now eapply dnf_closed_subst_eqnf.
+  - intros; rewrite <- qRun_subst; tea.
+    eapply LRTmEqIrrelevantCum'; [reflexivity|]; now unshelve eapply Hnil.
+  - rewrite <- qRun_subst; tea.
+    rewrite <- (qNat_subst _ σ).
+    eapply LRTmEqIrrelevantCum'; [reflexivity|]; now unshelve eapply Hval.
+  - rewrite <- (run_subst σ).
+    eapply LRTmRedIrrelevantCum'; [reflexivity|]; now unshelve eapply vrun.
+Qed.
 
-End ReflectValid.
+End StepEvalValid.
 
 Section ReflectCongValid.
 
@@ -1042,21 +1949,81 @@ Lemma StepCongValid :
   [Γ ||-v<l> u ≅ u' : tNat | vΓ | vNat ] ->
   [Γ ||-v<l> tStep t u ≅ tStep t' u' : tNat | vΓ | vNat ].
 Proof.
-Admitted.
+intros vtt' vuu'; constructor.
+intros; cbn.
+eapply StepRedEq.
++ irrelevance0; [reflexivity|]; now eapply vtt'.
++ irrelevance0; [reflexivity|]; now eapply vuu'.
++ destruct vrun as [vrun0 ?].
+  rewrite <- (run_subst σ).
+  irrelevance0; [reflexivity|]; now eapply vrun0.
+  Unshelve. all: tea.
+Qed.
+
+Notation totalValid := (TyCumValid (totalValid vΓ vrun vt vu)).
 
 Lemma totalCongValid :
   [Γ ||-v<l> t ≅ t' : arr tNat tNat | vΓ | vArr] ->
   [Γ ||-v<l> u ≅ u' : tNat | vΓ | vNat ] ->
-  [Γ ||-v<one> tTotal t u ≅ tTotal t' u' | vΓ | totalValid _ vrun vt vu ].
+  [Γ ||-v<one> tTotal t u ≅ tTotal t' u' | vΓ | totalValid ].
 Proof.
-intros; unfold tTotal.
-Admitted.
+intros vtt' vuu'; unfold tTotal.
+constructor; intros.
+pose (rNat := natRed (l := l) wfΔ).
+pose (rNatNat := SimpleArr.ArrRedTy rNat rNat).
+unshelve eapply ElURedEq; tea.
+rewrite !tEval_subst; cbn - [LRbuild].
+assert [rNatNat | Δ ||- t[σ] ≅ t'[σ] : tPNat].
+{ destruct vtt' as [rtt'].
+  unshelve eapply LRTmEqIrrelevantCum', rtt'; now tea. }
+assert [rNat | Δ ||- u[σ] ≅ u'[σ] : tNat].
+{ destruct vuu' as [ruu'].
+  unshelve eapply LRTmEqIrrelevantCum', ruu'; now tea. }
+unshelve eapply tEvalURedEq; tea.
++ unshelve eapply (SimpleArr.simple_appcongTerm (F := tNat)); eauto using SimpleArr.ArrRedTy.
+  - unshelve eapply (SimpleArr.simple_appcongTerm (F := tNat)); eauto using SimpleArr.ArrRedTy.
+    * apply reflLRTmEq.
+      destruct vrun as [rrun].
+      unshelve eapply LRTmRedIrrelevantCum', rrun; now tea.
+    * apply QuoteRed.
+      now unshelve eapply escapeEqTerm, reflLRTmEq, vt.
+    * apply QuoteRed.
+      unshelve eapply escapeEqTerm, reflLRTmEq; tea.
+      now eapply LRTmEqRed_r.
+    * eapply QuoteRedEq.
+      now eapply escapeEqTerm.
+  - now unshelve eapply LRTmRedIrrelevantCum', vu.
+  - now unshelve eapply LRTmRedIrrelevantCum', vu'.
++ eapply StepRedEq; tea.
+  rewrite <- (run_subst σ).
+  now unshelve eapply LRTmRedIrrelevantCum', vrun.
++ unshelve eapply (SimpleArr.simple_appcongTerm (F := tNat)); tea.
+  - now unshelve eapply LRTmRedIrrelevantCum', vu.
+  - now unshelve eapply LRTmRedIrrelevantCum', vu'.
+Qed.
 
 Lemma ReflectCongValid :
   [Γ ||-v<l> t ≅ t' : arr tNat tNat | vΓ | vArr] ->
   [Γ ||-v<l> u ≅ u' : tNat | vΓ | vNat ] ->
-  [Γ ||-v<one> tReflect t u ≅ tReflect t' u' : tTotal t u | vΓ | totalValid _ vrun vt vu ].
+  [Γ ||-v<one> tReflect t u ≅ tReflect t' u' : tTotal t u | vΓ | totalValid ].
 Proof.
-Admitted.
+intros vtt' vuu'; constructor; intros.
+pose (rNat := natRed (l := l) wfΔ).
+pose (rPNat := SimpleArr.ArrRedTy rNat rNat).
+assert (rtt' : [rPNat | Δ ||- t[σ] ≅ t'[σ] : tPNat]).
+{ unshelve eapply LRTmEqIrrelevantCum', vtt'; eauto. }
+assert (ruu' : [rNat | Δ ||- u[σ] ≅ u'[σ] : tNat]).
+{ unshelve eapply LRTmEqIrrelevantCum', vuu'; eauto. }
+cbn; unshelve eapply LRTmEqIrrelevantCum' with (lA := one), ReflectRedEq; tea.
++ eapply TotalRed.
+  - now unshelve eapply LRTmEqRed_l, rtt'.
+  - now unshelve eapply LRTmEqRed_l, ruu'.
+  - rewrite <- (run_subst σ).
+    now unshelve eapply LRTmRedIrrelevantCum', vrun.
++ now rewrite tTotal_subst.
++ now unshelve eapply LRTmEqIrrelevantCum', rtt'.
++ rewrite <- (run_subst σ).
+  now unshelve eapply LRTmRedIrrelevantCum', vrun.
+Qed.
 
 End ReflectCongValid.
