theories/Substitution/Introductions/Quote.v
@@ -8,11 +8,89 @@ From LogRel.Substitution.Introductions Require Import Universe Nat SimpleArr.
 Set Universe Polymorphism.
 Set Printing Primitive Projection Parameters.
 
+Section Utils. (* TODO: move me somewhere sensible *)
+
+Context `{GenericTypingProperties}.
+
+Lemma NatPropEq_diag {Γ A} {rNat : [Γ ||-Nat A]} :
+  (forall t u, [Γ ||-Nat t ≅ u : A | rNat] -> NatRedTm rNat t)
+  × (forall t u, NatPropEq rNat t u -> [Γ |- t : tNat] -> NatProp rNat t).
+Proof.
+apply NatRedEqInduction.
++ intros; econstructor; tea.
+  - now eapply lrefl.
+  - destruct redL; eauto.
++ constructor.
++ intros; now constructor.
++ intros * []; constructor.
+  constructor; tea; now eapply lrefl.
+Qed.
+
+Lemma LRTmEqRed_l : forall Γ l A t u (rA : [Γ ||-<l> A]),
+  [rA | Γ ||- t ≅ u : A] -> [rA | Γ ||- t : A].
+Proof.
+intros Γ l A t u rA.
+revert t u.
+pattern l, Γ, A, rA.
+eapply Induction.LR_rect_TyUr; clear l Γ A rA.
++ intros l Γ A rU t u [rl]; apply rl.
++ intros l Γ A rne t u [].
+  unshelve econstructor; [|tea|].
+  now eapply lrefl.
++ intros l Γ A rΠ IHdom IHcod t u []; tea.
++ intros l Γ A rNat t u [].
+  cbn; econstructor; [tea| |].
+  - now eapply lrefl.
+  - destruct redL; now eapply NatPropEq_diag.
++ intros l Γ A rEmpty t u [].
+  cbn; econstructor; [tea| |].
+  - now eapply lrefl.
+  - destruct prop; do 2 constructor.
+    * apply redL.
+    * destruct r; now eapply lrefl.
++ intros l Γ A rΣ IHdom IHcod t u []; tea.
++ intros l Γ A rId IHty IHty' t u [].
+  cbn; econstructor; [tea| |].
+  - now eapply lrefl.
+  - destruct prop; [left|right]; tea.
+    split; [apply redL|destruct r; now eapply lrefl].
+Qed.
+
+Lemma LRTmEqRed_r : forall Γ l A t u (rA : [Γ ||-<l> A]),
+  [rA | Γ ||- t ≅ u : A] -> [rA | Γ ||- u : A].
+Proof.
+intros; now eapply LRTmEqRed_l, LRTmEqSym.
+Qed.
+
+End Utils.
+
+Section QDnf.
+
+Lemma dnf_closed_subst_eqnf : forall t t₀ σ,
+  closed0 t -> dnf t -> [t[σ] ⇶* t₀] -> eqnf t[σ] t₀.
+Proof.
+intros; unfold eqnf.
+rewrite !erase_unannot_etared; f_equal.
+assert (Hrw : unannot t[σ] = unannot t) by now apply unannot_closed0_subst.
+eapply gredalg_unannot_dnf_id; [|tea].
+rewrite Hrw; now apply dnf_unannot.
+Qed.
+
+Lemma eqnf_closed0_subst : forall t σ, closed0 t -> eqnf t[σ] t.
+Proof.
+intros.
+unfold eqnf.
+rewrite !erase_unannot_etared; f_equal.
+now apply unannot_closed0_subst.
+Qed.
+
+End QDnf.
+
 Section QuoteValid.
 
 Context `{GenericTypingProperties}.
 
-Lemma qNatRed : forall {Γ A} (n : nat) (rA : [Γ ||-Nat A]), NatProp rA (qNat n).
+Lemma qNatRed0 : forall {Γ A} (n : nat) (rA : [Γ ||-Nat A]), NatProp rA (qNat n).
 Proof.
 intros Γ A n rA.
 induction n; cbn.
@@ -27,7 +105,18 @@ induction n; cbn.
   now apply convtm_qNat.
 Qed.
 
-Lemma qNatRedEq : forall {Γ A} (n : nat) (rA : [Γ ||-Nat A]), NatPropEq rA (qNat n) (qNat n).
+Lemma qNatRed {Γ l} (n : nat) (rNat : [Γ ||-<l> tNat]) : [rNat | Γ ||- qNat n : tNat].
+Proof.
+assert (rΓ : [|- Γ]).
+{ now eapply wfc_wft, escape. }
+pose (rNat' := natRed (l := l) rΓ).
+unshelve (irrelevance0; [reflexivity|]); [|apply rNat'|].
+cbn; econstructor; [| |apply qNatRed0].
+- now eapply redtmwf_refl, ty_qNat.
+- now eapply convtm_qNat.
+Qed.
+
+Lemma qNatRedEq0 : forall {Γ A} (n : nat) (rA : [Γ ||-Nat A]), NatPropEq rA (qNat n) (qNat n).
 Proof.
 intros Γ A n rA.
 induction n; cbn.
@@ -42,6 +131,15 @@ induction n; cbn.
   now apply convtm_qNat.
 Qed.
 
+Lemma qNatRedEq {Γ l} (n : nat) (rNat : [Γ ||-<l> tNat]) : [rNat | Γ ||- qNat n ≅ qNat n : tNat].
+Proof.
+assert [|- Γ] by now eapply wfc_wft, escape.
+unshelve (irrelevance0; [reflexivity|]); [apply l|now apply natRed|].
+induction n; cbn.
++ now unshelve eapply zeroRedEq.
++ eapply succRedEq; [| |tea]; apply qNatRed.
+Qed.
+
 Context {SN : SNTypingProperties ta _ _ _ _ _}.
 
 Lemma nf_eval : forall {l Γ A t} {vA : [Γ ||-<l> A]}, [vA | Γ ||- t : A] ->
@@ -54,15 +152,29 @@ destruct vt as (t₀&u₀&[]&[]&?&?&?).
 exists t₀; try now prod_splitter.
 Qed.
 
-  Lemma QuoteRedEq : forall Γ l t t' (rΓ : [|- Γ]) (rNat := natRed rΓ),
-    [Γ |- t : arr tNat tNat] ->
-    [Γ |- t' : arr tNat tNat] ->
-    [Γ ||-<l> t ≅ t' : arr tNat tNat | SimpleArr.ArrRedTy rNat rNat ] ->
+  Lemma QuoteEvalRedEq : forall Γ l t t₀ (rNat : [Γ ||-<l> tNat]),
+    [Γ |- t ≅ t₀ : tPNat] -> [t ⇶* t₀] -> dnf t₀ -> closed0 t₀ -> eqnf t t₀ ->
+    [Γ ||-<l> tQuote t ≅ qNat (model.(quote) (erase t)) : tNat | rNat ].
+  Proof.
+  intros.
+  eapply redSubstTerm.
+  + eapply qNatRed.
+  + transitivity (tQuote t₀).
+    - now apply redtm_quote.
+    - replace (erase t) with (erase t₀) by tea.
+      apply redtm_evalquote; tea.
+      now eapply urefl.
+  Qed.
+
+  Lemma QuoteRedEq : forall Γ l t t' (rNat : [Γ ||-<l> tNat]),
+    [Γ |- t ≅ t' : arr tNat tNat] ->
     [Γ ||-<l> tQuote t ≅ tQuote t' : tNat | rNat ].
   Proof.
-  intros * rt rt' re.
-  assert [Γ |- t ≅ t' : arr tNat tNat] by now eapply escapeEqTerm.
-  apply escapeEqTerm, snty_nf in re.
+  intros * rtt'.
+  assert (rΓ : [|- Γ]) by now eapply wfc_wft, escape.
+  unshelve (irrelevance0; [reflexivity|]); [tea|now apply natRed|].
+  assert (re : [Γ |- t ≅ t' : arr tNat tNat]) by eauto.
+  apply snty_nf in re.
   destruct re as (l₀&r₀&[]&[]&?&?&?).
   remember (is_closedn 0 l₀) as b eqn:Hc; symmetry in Hc.
   assert (Hc' : is_closedn 0 r₀ = b).
@@ -82,11 +194,11 @@ Qed.
         apply redtm_evalquote; tea.
         now eapply urefl.
     + now apply convtm_qNat.
-    + apply qNatRedEq.
+    + apply qNatRedEq0.
   - assert [Γ |-[ ta ] tQuote l₀ ~ tQuote r₀ : tNat].
     { apply convneu_quote; tea.
-      + etransitivity; [now symmetry|].
-        etransitivity; tea.
+      + transitivity t; [now symmetry|].
+        transitivity t'; tea.
       + unfold closed0; destruct is_closedn; cbn; congruence.
       + unfold closed0; destruct is_closedn; cbn; congruence. }
     exists (tQuote l₀) (tQuote r₀).
@@ -96,6 +208,14 @@ Qed.
       apply redtm_quote; tea.
     + apply convtm_convneu; tea.
     + constructor; constructor; tea.
+  Qed.
+
+  Lemma QuoteRed : forall Γ l t (rNat : [Γ ||-<l> tNat]),
+    [Γ |- t ≅ t : arr tNat tNat] ->
+    [Γ ||-<l> tQuote t : tNat | rNat ].
+  Proof.
+    intros.
+    now eapply LRTmEqRed_l, QuoteRedEq.
   Qed.
 
   Context {Γ l t} (vΓ : [||-v Γ])
@@ -121,7 +241,7 @@ Qed.
       { now apply ty_quote. }
       pose (c := is_closedn 0 r); assert (is_closedn 0 r = c) as Hc by reflexivity; destruct c.
       + pose (q := qNat (model.(quote) (erase r))).
-        exists q; [|now apply convtm_qNat|apply qNatRed].
+        exists q; [|now apply convtm_qNat|apply qNatRed0].
         constructor.
         { now apply ty_qNat. }
         { transitivity (tQuote r); [tea|].
@@ -134,14 +254,13 @@ Qed.
         * apply convtm_convneu, convneu_quote; tea.
         * apply NatRedTm.neR; constructor; tea.
           now apply convneu_quote.
-  - intros Δ σ σ' tΔ vσ vσ' vσσ'; cbn.
+  - intros Δ σ σ' tΔ vσ vσ' vσσ'.
     destruct vt as [vt0 vte].
     assert [Δ |- t[σ] : arr tNat tNat].
     { unshelve eapply escapeTerm, vt0; tea. }
     assert [Δ |- t[σ'] : arr tNat tNat].
     { unshelve eapply escapeTerm, vt0; tea. }
-    unshelve eapply QuoteRedEq, LRTmEqIrrelevant', vte; cbn; tea.
-    reflexivity.
+    unshelve eapply QuoteRedEq, escapeEqTerm, vte; cbn; tea.
   Qed.
 
 Lemma evalQuoteValid : dnf t -> closed0 t ->
@@ -169,12 +288,9 @@ exists q q; cbn in *.
 - constructor; [now apply ty_qNat|].
   rewrite quote_subst; [|tea].
   replace (erase t[σ]) with (erase t₀); [now apply redtm_refl, ty_qNat|].
-  rewrite !erase_unannot_etared; f_equal.
-  assert (Hrw : unannot t[σ] = unannot t) by now apply unannot_closed0_subst.
-  symmetry; eapply gredalg_unannot_dnf_id; [|tea].
-  rewrite Hrw; now apply dnf_unannot.
+  symmetry; now apply dnf_closed_subst_eqnf.
 - now apply convtm_qNat.
-- now apply qNatRedEq.
+- now apply qNatRedEq0.
 Qed.
 
 End QuoteValid.
@@ -197,13 +313,12 @@ Lemma QuoteCongValid :
   [Γ ||-v<l> tQuote t ≅ tQuote t' : tNat | vΓ | vNat].
 Proof.
 intros [vte]; constructor.
-intros Δ σ tΔ vσ; cbn.
+intros Δ σ tΔ vσ.
 assert [Δ |- t[σ] : arr tNat tNat].
 { unshelve eapply escapeTerm, vt; tea. }
 assert [Δ |- t'[σ] : arr tNat tNat].
 { unshelve eapply escapeTerm, vt'; tea. }
-unshelve eapply QuoteRedEq, LRTmEqIrrelevant', vte; cbn; tea.
-reflexivity.
+unshelve eapply QuoteRedEq, escapeEqTerm, vte; cbn; tea.
 Qed.
 
 End QuoteCongValid.
